#193 #207 fixed all comments that were generator-related and re-generated

abp/ReceiverAutomaton.thy
@@ -3,12 +3,24 @@
  * This file was generated from Receiver.maa and will be overridden when changed. To change
  * permanently, consider changing the model itself.
  *
- * Generated on Sep 21, 2018 4:47:19 PM by isartransformer 1.0.0
+ * Generated on Sep 22, 2018 1:11:51 PM by isartransformer 1.0.0
  *)
 theory ReceiverAutomaton
   imports bundle.tsynBundle automat.dAutomaton
 
 begin
+
+
+(* TODO SWS: Move this to dAutomaton *)
+lemma da_h_stepI:
+  assumes "sbeDom sbe = daDom da"
+      and "(daNextOutput da s sbe) = out"
+      and "(daNextState da s sbe) = nextState"
+  shows "spfConcIn (sbe2SB sbe)\<cdot>(da_h da s) = spfConcOut out\<cdot>(da_h da nextState)"
+  by (metis (no_types) assms da_h_dom da_h_final_h3 spfConcIn_dom spfConcIn_step spfConcOut_dom spf_eq)
+
+(* TODO SWS: Move this to...? *)
+setup_lifting type_definition_cfun
 
 (* Helper for easier generation *)
 fun prepend :: "'a::type list \<Rightarrow> 'a \<Rightarrow> 'a list" where
@@ -17,41 +29,41 @@ fun prepend :: "'a::type list \<Rightarrow> 'a \<Rightarrow> 'a list" where
 section \<open>Datatype definition\<close>
 
 datatype receiverMessage = ReceiverPair_ReceiverNat_ReceiverBool "(nat\<times>bool)" | ReceiverBool "bool" | ReceiverNat "nat"
+
 instance receiverMessage :: countable
   apply(intro_classes)
   by(countable_datatype)
 
 instantiation receiverMessage :: message
 begin
-  fun ctype_receiverMessage :: "channel  \<Rightarrow> receiverMessage set" where
+  fun ctype_receiverMessage :: "channel \<Rightarrow> receiverMessage set" where
   "ctype_receiverMessage c = (
     if c = \<C> ''dr'' then range ReceiverPair_ReceiverNat_ReceiverBool else
     if c = \<C> ''ar'' then range ReceiverBool else
     if c = \<C> ''o'' then range ReceiverNat else
-    undefined)" (* SWS: undefined is better, otherwise "time" is allowed on the other channels *)
-    instance
+    undefined)"
+  instance
     by(intro_classes)
 end
 
 
 section \<open>Helpers to create a bundle from a single raw element\<close>
 
-(* SWS: I think it is better to write the channel-name excatly like in the MAA-Model, so "dr" instead of "Dr" *)
-lift_definition receiverElem_raw_Dr :: "(nat\<times>bool) \<Rightarrow> receiverMessage tsyn sbElem" is
+lift_definition receiverElem_raw_dr :: "(nat\<times>bool) \<Rightarrow> receiverMessage tsyn sbElem" is
 "\<lambda>x. [\<C> ''dr'' \<mapsto> Msg (ReceiverPair_ReceiverNat_ReceiverBool x)]"
   unfolding sbElemWell_def
   unfolding usclOkay_stream_def
   unfolding ctype_tsyn_def
   by simp
 
-lift_definition receiverElem_raw_Ar :: "bool \<Rightarrow> receiverMessage tsyn sbElem" is
+lift_definition receiverElem_raw_ar :: "bool \<Rightarrow> receiverMessage tsyn sbElem" is
 "\<lambda>x. [\<C> ''ar'' \<mapsto> Msg (ReceiverBool x)]"
   unfolding sbElemWell_def
   unfolding usclOkay_stream_def
   unfolding ctype_tsyn_def
   by simp
 
-lift_definition receiverElem_raw_O :: "nat \<Rightarrow> receiverMessage tsyn sbElem" is
+lift_definition receiverElem_raw_o :: "nat \<Rightarrow> receiverMessage tsyn sbElem" is
 "\<lambda>x. [\<C> ''o'' \<mapsto> Msg (ReceiverNat x)]"
   unfolding sbElemWell_def
   unfolding usclOkay_stream_def
@@ -61,131 +73,136 @@ lift_definition receiverElem_raw_O :: "nat \<Rightarrow> receiverMessage tsyn sb
 
 section \<open>Helpers to create a bundle from a single tsyn element\<close>
 
-fun receiverElem_Dr :: "(nat\<times>bool) tsyn \<Rightarrow> receiverMessage tsyn sbElem" where
-"receiverElem_Dr (Msg port_dr) = receiverElem_raw_Dr port_dr" |
-"receiverElem_Dr null = sbeNull {\<C> ''dr''}"
-(* SWS: Remove from simps *)
+fun receiverElem_dr :: "(nat\<times>bool) tsyn \<Rightarrow> receiverMessage tsyn sbElem" where
+"receiverElem_dr (Msg port_dr) = receiverElem_raw_dr port_dr" |
+"receiverElem_dr null = sbeNull {\<C> ''dr''}"
 
-definition receiver_Dr :: "(nat\<times>bool) tsyn \<Rightarrow> receiverMessage tsyn SB" where
-"receiver_Dr port_dr = sbe2SB (receiverElem_Dr port_dr)"
+declare receiverElem_dr.simps[simp del]
 
-fun receiverElem_Ar :: "bool tsyn \<Rightarrow> receiverMessage tsyn sbElem" where
-"receiverElem_Ar (Msg port_ar) = receiverElem_raw_Ar port_ar" |
-"receiverElem_Ar null = sbeNull {\<C> ''ar''}"
+definition receiver_dr :: "(nat\<times>bool) tsyn \<Rightarrow> receiverMessage tsyn SB" where
+"receiver_dr port_dr = sbe2SB (receiverElem_dr port_dr)"
 
-definition receiver_Ar :: "bool tsyn \<Rightarrow> receiverMessage tsyn SB" where
-"receiver_Ar port_ar = sbe2SB (receiverElem_Ar port_ar)"
+fun receiverElem_ar :: "bool tsyn \<Rightarrow> receiverMessage tsyn sbElem" where
+"receiverElem_ar (Msg port_ar) = receiverElem_raw_ar port_ar" |
+"receiverElem_ar null = sbeNull {\<C> ''ar''}"
 
-fun receiverElem_O :: "nat tsyn \<Rightarrow> receiverMessage tsyn sbElem" where
-"receiverElem_O (Msg port_o) = receiverElem_raw_O port_o" |
-"receiverElem_O null = sbeNull {\<C> ''o''}"
+declare receiverElem_ar.simps[simp del]
 
-definition receiver_O :: "nat tsyn \<Rightarrow> receiverMessage tsyn SB" where
-"receiver_O port_o = sbe2SB (receiverElem_O port_o)"
+definition receiver_ar :: "bool tsyn \<Rightarrow> receiverMessage tsyn SB" where
+"receiver_ar port_ar = sbe2SB (receiverElem_ar port_ar)"
+
+fun receiverElem_o :: "nat tsyn \<Rightarrow> receiverMessage tsyn sbElem" where
+"receiverElem_o (Msg port_o) = receiverElem_raw_o port_o" |
+"receiverElem_o null = sbeNull {\<C> ''o''}"
+
+declare receiverElem_o.simps[simp del]
+
+definition receiver_o :: "nat tsyn \<Rightarrow> receiverMessage tsyn SB" where
+"receiver_o port_o = sbe2SB (receiverElem_o port_o)"
 
 (* Create one sbElem for all input channels *)
-
-(* SWS: use "definition" as default instead of "fun". Because "fun" adds the stuff to the simplifier.
-      If you need rekursion still fun *)
-definition receiverElemIn_Dr :: "(nat\<times>bool) tsyn \<Rightarrow> receiverMessage tsyn sbElem" where
-"receiverElemIn_Dr port_dr = (receiverElem_Dr port_dr)"
+definition receiverElemIn_dr :: "(nat\<times>bool) tsyn \<Rightarrow> receiverMessage tsyn sbElem" where
+"receiverElemIn_dr port_dr = (receiverElem_dr port_dr)"
 
 (* Create one sbElem for all output channels *)
-definition receiverElemOut_Ar_O :: "bool tsyn \<Rightarrow> nat tsyn \<Rightarrow> receiverMessage tsyn sbElem" where
-"receiverElemOut_Ar_O port_ar port_o = (receiverElem_Ar port_ar) \<plusminus> (receiverElem_O port_o)"
+definition receiverElemOut_ar_o :: "bool tsyn \<Rightarrow> nat tsyn \<Rightarrow> receiverMessage tsyn sbElem" where
+"receiverElemOut_ar_o port_ar port_o = (receiverElem_ar port_ar) \<plusminus> (receiverElem_o port_o)"
 
 (* Create one SB for all input channels *)
-fun receiverIn_Dr :: "(nat\<times>bool) tsyn \<Rightarrow> receiverMessage tsyn SB" where
-"receiverIn_Dr port_dr = (sbe2SB (receiverElemIn_Dr port_dr))"
+definition receiverIn_dr :: "(nat\<times>bool) tsyn \<Rightarrow> receiverMessage tsyn SB" where
+"receiverIn_dr port_dr = (sbe2SB (receiverElemIn_dr port_dr))"
 
 (* Create one SB for all output channels *)
-fun receiverOut_Ar_O :: "bool tsyn \<Rightarrow> nat tsyn \<Rightarrow> receiverMessage tsyn SB" where
-"receiverOut_Ar_O port_ar port_o = (sbe2SB (receiverElemOut_Ar_O port_ar port_o))"
+definition receiverOut_ar_o :: "bool tsyn \<Rightarrow> nat tsyn \<Rightarrow> receiverMessage tsyn SB" where
+"receiverOut_ar_o port_ar port_o = (sbe2SB (receiverElemOut_ar_o port_ar port_o))"
 
 
 section \<open>Helpers to create a bundle from a tsyn list of elements\<close>
 
-fun receiver_list_Dr :: "((nat\<times>bool) tsyn) list \<Rightarrow> receiverMessage tsyn SB" where
-"receiver_list_Dr (x#xs) = ubConcEq (receiver_Dr x)\<cdot>(receiver_list_Dr xs)" |
-"receiver_list_Dr []     = ubLeast {\<C> ''dr''}"
+fun receiver_list_dr :: "((nat\<times>bool) tsyn) list \<Rightarrow> receiverMessage tsyn SB" where
+"receiver_list_dr (x#xs) = ubConcEq (receiver_dr x)\<cdot>(receiver_list_dr xs)" |
+"receiver_list_dr []     = ubLeast {\<C> ''dr''}"
 
-fun receiver_list_Ar :: "(bool tsyn) list \<Rightarrow> receiverMessage tsyn SB" where
-"receiver_list_Ar (x#xs) = ubConcEq (receiver_Ar x)\<cdot>(receiver_list_Ar xs)" |
-"receiver_list_Ar []     = ubLeast {\<C> ''ar''}"
+fun receiver_list_ar :: "(bool tsyn) list \<Rightarrow> receiverMessage tsyn SB" where
+"receiver_list_ar (x#xs) = ubConcEq (receiver_ar x)\<cdot>(receiver_list_ar xs)" |
+"receiver_list_ar []     = ubLeast {\<C> ''ar''}"
 
-fun receiver_list_O :: "(nat tsyn) list \<Rightarrow> receiverMessage tsyn SB" where
-"receiver_list_O (x#xs) = ubConcEq (receiver_O x)\<cdot>(receiver_list_O xs)" |
-"receiver_list_O []     = ubLeast {\<C> ''o''}"
+fun receiver_list_o :: "(nat tsyn) list \<Rightarrow> receiverMessage tsyn SB" where
+"receiver_list_o (x#xs) = ubConcEq (receiver_o x)\<cdot>(receiver_list_o xs)" |
+"receiver_list_o []     = ubLeast {\<C> ''o''}"
 
 (* Create one SB for all input channels *)
-(* "definition" instead of "fun" *)
-fun receiverIn_list_Dr :: "(nat\<times>bool) tsyn list \<Rightarrow> receiverMessage tsyn SB" where
-"receiverIn_list_Dr port_dr = (receiver_list_Dr port_dr)"
+definition receiverIn_list_dr :: "(nat\<times>bool) tsyn list \<Rightarrow> receiverMessage tsyn SB" where
+"receiverIn_list_dr port_dr = (receiver_list_dr port_dr)"
 
 (* Create one SB for all output channels *)
-fun receiverOut_list_Ar_O :: "bool tsyn list \<Rightarrow> nat tsyn list \<Rightarrow> receiverMessage tsyn SB" where
-"receiverOut_list_Ar_O port_ar port_o = (receiver_list_Ar port_ar) \<uplus> (receiver_list_O port_o)"
+definition receiverOut_list_ar_o :: "bool tsyn list \<Rightarrow> nat tsyn list \<Rightarrow> receiverMessage tsyn SB" where
+"receiverOut_list_ar_o port_ar port_o = (receiver_list_ar port_ar) \<uplus> (receiver_list_o port_o)"
 
 
 section \<open>Helpers to create a bundle from a tsyn stream of elements\<close>
 
-(* SWS: Setter-helper. should be invisible. Could also be done in one definition but then we cannot use lift_definition *)
-lift_definition receiver_stream_Dr_h :: "((nat\<times>bool)) tsyn stream \<Rightarrow> receiverMessage tsyn SB" is
+lift_definition receiver_stream_dr_h :: "(nat\<times>bool) tsyn stream \<Rightarrow> receiverMessage tsyn SB" is
 "\<lambda> s. [(\<C> ''dr'') \<mapsto> (tsynMap (ReceiverPair_ReceiverNat_ReceiverBool)\<cdot>s)]"
   unfolding ubWell_def usclOkay_stream_def ctype_tsyn_def
   apply auto
-  sorry 
-(* SWS: letzter Teil des Beweises braucht einen allgemeinen Beweis damit das autogenerieren nicht zu komplex wird. 
-     Kommt später, erstmal sorry *)
+  sorry
 
-(* SWS: this is a general stuff, should go to prelude / not autogenerated *)
-setup_lifting type_definition_cfun
+lift_definition receiver_stream_dr :: "((nat\<times>bool)) tsyn stream \<rightarrow> receiverMessage tsyn SB" is
+"receiver_stream_dr_h"
+  sorry
 
-lift_definition receiver_stream_Dr :: "((nat\<times>bool)) tsyn stream \<rightarrow> receiverMessage tsyn SB" is
-"receiver_stream_Dr_h"
-  sorry (* SWS: No fucking clue how to proof this ... *)
+lift_definition receiver_stream_ar_h :: "bool tsyn stream \<Rightarrow> receiverMessage tsyn SB" is
+"\<lambda> s. [(\<C> ''ar'') \<mapsto> (tsynMap (ReceiverBool)\<cdot>s)]"
+  unfolding ubWell_def usclOkay_stream_def ctype_tsyn_def
+  apply auto
+  sorry
 
+lift_definition receiver_stream_ar :: "(bool) tsyn stream \<rightarrow> receiverMessage tsyn SB" is
+"receiver_stream_ar_h"
+  sorry
 
-definition receiver_stream_Ar :: "(bool) tsyn stream \<rightarrow> receiverMessage tsyn SB" where
-"receiver_stream_Ar = undefined"  (* SWS: Analog zu oben, habs schonmal cont gemacht um die multi-parameter zu testen *)
+lift_definition receiver_stream_o_h :: "nat tsyn stream \<Rightarrow> receiverMessage tsyn SB" is
+"\<lambda> s. [(\<C> ''o'') \<mapsto> (tsynMap (ReceiverNat)\<cdot>s)]"
+  unfolding ubWell_def usclOkay_stream_def ctype_tsyn_def
+  apply auto
+  sorry
 
-definition receiver_stream_O :: "(nat) tsyn stream \<rightarrow> receiverMessage tsyn SB" where
-"receiver_stream_O = undefined"
+lift_definition receiver_stream_o :: "(nat) tsyn stream \<rightarrow> receiverMessage tsyn SB" is
+"receiver_stream_o_h"
+  sorry
 
 (* Create one SB for all input channels *)
-definition receiverIn_stream_Dr :: "(nat\<times>bool) tsyn stream \<rightarrow> receiverMessage tsyn SB" where
-"receiverIn_stream_Dr = (\<Lambda> port_dr. receiver_stream_Dr\<cdot>port_dr)"
-  
+definition receiverIn_stream_dr :: "(nat\<times>bool) tsyn stream \<rightarrow> receiverMessage tsyn SB" where
+"receiverIn_stream_dr = (\<Lambda>  port_dr. (receiver_stream_dr\<cdot>port_dr))"
+
 (* Create one SB for all output channels *)
-(* SWS: Ich würde hier gerne lift_definition verewnden, aber das erzeugt RICHTIG hässliche beweise bei mehreren parametern *)
-(* SWS: vllt muss man dafür noch extra cont-lemma generieren :/ *)
-definition receiverOut_stream_Ar_O :: "bool tsyn stream \<rightarrow> nat tsyn stream \<rightarrow> receiverMessage tsyn SB" where
-"receiverOut_stream_Ar_O  = (\<Lambda> port_ar port_o. (receiver_stream_Ar\<cdot>port_ar) \<uplus> (receiver_stream_O\<cdot>port_o))"
+definition receiverOut_stream_ar_o :: "bool tsyn stream \<rightarrow> nat tsyn stream \<rightarrow> receiverMessage tsyn SB" where
+"receiverOut_stream_ar_o = (\<Lambda>  port_ar port_o. (receiver_stream_ar\<cdot>port_ar) \<uplus> (receiver_stream_o\<cdot>port_o))"
 
 
 section \<open>Helpers to get tsyn elements and streams from sbElems and SBs\<close>
 
+fun receiverElem_get_dr :: "receiverMessage tsyn sbElem \<Rightarrow> ((nat\<times>bool)) tsyn" where
+"receiverElem_get_dr sbe = undefined"
 
-fun receiverElem_get_Dr :: "receiverMessage tsyn sbElem \<Rightarrow> ((nat\<times>bool)) tsyn" where
-"receiverElem_get_Dr sbe = undefined" (* SWS: das braucht noch eine allgemein definition über "tsyn" *)
-
-(* SWS: Das ist kein Elem, renaming zu "receiver_get_stream_Dr" *)
-lift_definition receiverElem_get_stream_Dr :: "receiverMessage tsyn SB \<rightarrow> ((nat\<times>bool)) tsyn stream" is
+lift_definition receiver_get_stream_dr :: "receiverMessage tsyn SB \<rightarrow> (nat\<times>bool) tsyn stream" is
 "\<lambda>sb. tsynMap (inv ReceiverPair_ReceiverNat_ReceiverBool)\<cdot>(sb . (\<C> ''dr''))"
-  by(simp add: cfun_def)  (* SWS: das lief doch schön! *)
+  by(simp add: cfun_def)
 
-fun receiverElem_get_Ar :: "receiverMessage tsyn sbElem \<Rightarrow> (bool) tsyn" where
-"receiverElem_get_Ar sbe = undefined"
+fun receiverElem_get_ar :: "receiverMessage tsyn sbElem \<Rightarrow> (bool) tsyn" where
+"receiverElem_get_ar sbe = undefined"
 
-fun receiverElem_get_stream_Ar :: "receiverMessage tsyn SB \<Rightarrow> (bool) tsyn stream" where
-"receiverElem_get_stream_Ar sb = undefined"
+lift_definition receiver_get_stream_ar :: "receiverMessage tsyn SB \<rightarrow> bool tsyn stream" is
+"\<lambda>sb. tsynMap (inv ReceiverBool)\<cdot>(sb . (\<C> ''ar''))"
+  by(simp add: cfun_def)
 
-fun receiverElem_get_O :: "receiverMessage tsyn sbElem \<Rightarrow> (nat) tsyn" where
-"receiverElem_get_O sbe = undefined"
+fun receiverElem_get_o :: "receiverMessage tsyn sbElem \<Rightarrow> (nat) tsyn" where
+"receiverElem_get_o sbe = undefined"
 
-fun receiverElem_get_stream_O :: "receiverMessage tsyn SB \<Rightarrow> (nat) tsyn stream" where
-"receiverElem_get_stream_O sb = undefined"
-
+lift_definition receiver_get_stream_o :: "receiverMessage tsyn SB \<rightarrow> nat tsyn stream" is
+"\<lambda>sb. tsynMap (inv ReceiverNat)\<cdot>(sb . (\<C> ''o''))"
+  by(simp add: cfun_def)
 
 
 
@@ -204,20 +221,20 @@ fun getReceiverSubState :: "ReceiverState \<Rightarrow> ReceiverSubstate" where
 (* Helper that allows us to utilize pattern matching *)
 fun receiverTransitionH :: "(ReceiverState \<times> ((nat\<times>bool) tsyn)) \<Rightarrow> (ReceiverState \<times> receiverMessage tsyn SB)" where
 "receiverTransitionH (ReceiverState Rf, (\<^cancel>\<open>dr\<mapsto>\<close>Msg port_dr)) =
-  (if((snd port_dr)=True) then ((ReceiverState Rf, (receiverOut_Ar_O (Msg (True)) null)))
-   else if((snd port_dr)=False) then ((ReceiverState Rt, (receiverOut_Ar_O (Msg (False)) (Msg ((fst port_dr))))))
-   else (ReceiverState Rf, (receiverOut_Ar_O null null)))" |
+  (if((snd port_dr)=True) then ((ReceiverState Rf, (receiverOut_ar_o (Msg (True)) null)))
+   else if((snd port_dr)=False) then ((ReceiverState Rt, (receiverOut_ar_o (Msg (False)) (Msg ((fst port_dr))))))
+   else (ReceiverState Rf, (receiverOut_ar_o null null)))" |
 
 "receiverTransitionH (ReceiverState Rf, (\<^cancel>\<open>dr\<mapsto>\<close>null)) =
-  (ReceiverState Rf, (receiverOut_Ar_O null null))" |
+  (ReceiverState Rf, (receiverOut_ar_o null null))" |
 
 "receiverTransitionH (ReceiverState Rt, (\<^cancel>\<open>dr\<mapsto>\<close>Msg port_dr)) =
-  (if((snd port_dr)=True) then ((ReceiverState Rf, (receiverOut_Ar_O (Msg (True)) (Msg ((fst port_dr))))))
-   else if((snd port_dr)=False) then ((ReceiverState Rt, (receiverOut_Ar_O (Msg (False)) null)))
-   else (ReceiverState Rt, (receiverOut_Ar_O null null)))" |
+  (if((snd port_dr)=True) then ((ReceiverState Rf, (receiverOut_ar_o (Msg (True)) (Msg ((fst port_dr))))))
+   else if((snd port_dr)=False) then ((ReceiverState Rt, (receiverOut_ar_o (Msg (False)) null)))
+   else (ReceiverState Rt, (receiverOut_ar_o null null)))" |
 
 "receiverTransitionH (ReceiverState Rt, (\<^cancel>\<open>dr\<mapsto>\<close>null)) =
-  (ReceiverState Rt, (receiverOut_Ar_O null null))"
+  (ReceiverState Rt, (receiverOut_ar_o null null))"
 
 (* Domain *)
 definition receiverDom :: "channel set" where
@@ -229,159 +246,212 @@ definition receiverRan :: "channel set" where
 
 (* Transition function *)
 definition receiverTransition :: "(ReceiverState \<times> receiverMessage tsyn sbElem) \<Rightarrow> (ReceiverState \<times> receiverMessage tsyn SB)" where
-"receiverTransition  = (\<lambda> (s,b). (if (sbeDom b) = receiverDom then receiverTransitionH (s, (receiverElem_get_Dr b)) else undefined))"
+"receiverTransition = (\<lambda> (s,b). (if (sbeDom b) = receiverDom then receiverTransitionH (s, (receiverElem_get_dr b)) else undefined))"
+
+(* Initial state *)
+definition receiverInitialState :: "ReceiverState" where
+"receiverInitialState = ReceiverState Rt "
+
+(* Initial output *)
+definition receiverInitialOutput :: "receiverMessage tsyn SB" where
+"receiverInitialOutput = receiverOut_ar_o null null"
 
 (* The final automaton *)
-(* SWS: kleiner Anfangsbuchstabe wie überall sonst auch *)
-lift_definition ReceiverAutomaton :: "(ReceiverState, receiverMessage tsyn) dAutomaton" is
-"(receiverTransition, ReceiverState Rt , (receiverOut_Ar_O null null), receiverDom, receiverRan)"
+lift_definition receiverAutomaton :: "(ReceiverState, receiverMessage tsyn) dAutomaton" is
+"(receiverTransition, receiverInitialState, receiverInitialOutput, receiverDom, receiverRan)"
   by (simp add: receiverDom_def receiverRan_def)
 
-(* SWS: kleiner Anfangsbuchstabe wie überall sonst auch *)
 (* Stream processing function for each state (handy for step lemmata) *)
-definition ReceiverStep :: "(ReceiverState \<Rightarrow> (receiverMessage tsyn, receiverMessage tsyn) SPF)" where
-"ReceiverStep = da_h ReceiverAutomaton"
+definition receiverStep :: "(ReceiverState \<Rightarrow> (receiverMessage tsyn, receiverMessage tsyn) SPF)" where
+"receiverStep = da_h receiverAutomaton"
 
 (* The final SPF *)
-(* SWS: kleiner Anfangsbuchstabe wie überall sonst auch *)
-definition ReceiverSPF :: "(receiverMessage tsyn, receiverMessage tsyn) SPF" where
-"ReceiverSPF = da_H ReceiverAutomaton"
+definition receiverSPF :: "(receiverMessage tsyn, receiverMessage tsyn) SPF" where
+"receiverSPF = da_H receiverAutomaton"
 
 
+section \<open>Lemmas for automaton definition\<close>
 
-(* SWS: this is unrelated from the automaton. Can be before the entire automaton definition *)
-section \<open>Lemma over the Datatype-Definitions\<close>
-
-lemma receiverelemin_dom[simp]: "sbeDom (receiverElemIn_Dr port_dr) = receiverDom"
-  sorry (* SWS: Analog für ran *)
-
-lemma receiverin_dom[simp]: "ubDom\<cdot>(receiverIn_Dr port_dr) = receiverDom"
-  sorry (* SWS: Analog für ran *)
-
-lemma receiverelem_dr_id[simp]: "receiverElem_get_Dr (receiverElem_Dr port_dr) = port_dr"
-  sorry (* SWS: Analog die gleichen "get von set" lemma über Bundle *)
-
-lemma receiverelemin_dr_id[simp]: "receiverElem_get_Dr (receiverElemIn_Dr port_dr) = port_dr"
-  sorry (* SWS: Analog die gleichen "get von set" lemma über Bundle *)
-
-
-
-(* SWS: Very general lemma over the definition *)
-
-lemma receiveraut_trans[simp]: "daTransition ReceiverAutomaton = receiverTransition"
+lemma receiverautomaton_trans[simp]: "daTransition receiverAutomaton = receiverTransition"
   sorry
-lemma receiveraut_dom [simp]: "daDom ReceiverAutomaton = receiverDom"
+
+lemma receiverautomaton_initialstate[simp]: "daInitialState receiverAutomaton = receiverInitialState"
   sorry
-(* SWS: Das gleiche für alle Elemente des Tupels/für alle "daXXXX" definitionen *)
+
+lemma receiverautomaton_initialoutput[simp]: "daInitialOutput receiverAutomaton = receiverInitialOutput"
+  sorry
+
+lemma receiverautomaton_dom[simp]: "daDom receiverAutomaton = receiverDom"
+  sorry
+
+lemma receiverautomaton_ran[simp]: "daRan receiverAutomaton = receiverRan"
+  sorry
+
+
+section \<open>Lemmas for single tsyn setter\<close>
+
+lemma receiverelemin_dr_dom[simp]: "sbeDom (receiverElemIn_dr port_dr) = receiverDom"
+  sorry
+
+lemma receiverelemout_ar_o_dom[simp]: "sbeDom (receiverElemOut_ar_o port_ar port_o) = receiverRan"
+  sorry
+
+lemma receiverin_dr_dom[simp]: "ubDom\<cdot>(receiverIn_dr port_dr) = receiverDom"
+  sorry
+
+lemma receiverout_ar_o_dom[simp]: "ubDom\<cdot>(receiverOut_ar_o port_ar port_o) = receiverRan"
+  sorry
+
+
+section \<open>Lemmas for getter\<close>
+
+lemma receiverelem_dr_id[simp]: "receiverElem_get_dr (receiverElem_dr port_dr) = port_dr"
+  sorry
+
+lemma receiver_stream_dr_id[simp]: "receiver_get_stream_dr\<cdot>(receiver_stream_dr\<cdot>port_dr) = port_dr"
+  sorry
+
+lemma receiverelem_ar_id[simp]: "receiverElem_get_ar (receiverElem_ar port_ar) = port_ar"
+  sorry
+
+lemma receiver_stream_ar_id[simp]: "receiver_get_stream_ar\<cdot>(receiver_stream_ar\<cdot>port_ar) = port_ar"
+  sorry
+
+lemma receiverelem_o_id[simp]: "receiverElem_get_o (receiverElem_o port_o) = port_o"
+  sorry
+
+lemma receiver_stream_o_id[simp]: "receiver_get_stream_o\<cdot>(receiver_stream_o\<cdot>port_o) = port_o"
+  sorry
 
 
 section \<open>Step-wise lemmata for the transition function\<close>
 
-(* SWS: automaton-name in die lemma *)
 (* Line 18:  Rf -> Rf [dr.snd=true] / {ar=true}; *)
-lemma transition_0_0 [simp]:
+lemma receiverTransition_0_0[simp]:
   assumes "(snd port_dr)=True"
-    shows "receiverTransition ((ReceiverState Rf ), (receiverElemIn_Dr (Msg port_dr)))
-         = (ReceiverState Rf, (receiverOut_Ar_O (Msg (True)) null))"
-  apply(simp add: receiverTransition_def) (* SWS: i will continue to proof this after more lemma/definitions are there *)
+    shows "receiverTransition ((ReceiverState Rf ), (receiverElemIn_dr (Msg port_dr)))
+         = (ReceiverState Rf, (receiverOut_ar_o (Msg (True)) null))"
+  apply(simp add: receiverTransition_def)
   sorry
 
 (* Line 19:  Rf -> Rt [dr.snd=false] / {ar=false, o=dr.fst}; *)
-lemma transition_0_1:
+lemma receiverTransition_0_1[simp]:
   assumes "(snd port_dr)=False"
-    shows "receiverTransition ((ReceiverState Rf ), (receiverElemIn_Dr (Msg port_dr)))
-         = (ReceiverState Rt, (receiverOut_Ar_O (Msg (False)) (Msg ((fst port_dr)))))"
-  oops
+    shows "receiverTransition ((ReceiverState Rf ), (receiverElemIn_dr (Msg port_dr)))
+         = (ReceiverState Rt, (receiverOut_ar_o (Msg (False)) (Msg ((fst port_dr)))))"
+  apply(simp add: receiverTransition_def)
+  sorry
 
 (* Line 17:  Rf -> Rf {dr==null}; *)
-lemma transition_1_0:
+lemma receiverTransition_1_0[simp]:
   assumes "True"
-    shows "receiverTransition ((ReceiverState Rf ), (receiverElemIn_Dr null))
-         = (ReceiverState Rf, (receiverOut_Ar_O null null))"
-  oops
+    shows "receiverTransition ((ReceiverState Rf ), (receiverElemIn_dr null))
+         = (ReceiverState Rf, (receiverOut_ar_o null null))"
+  apply(simp add: receiverTransition_def)
+  sorry
 
 (* Line 14:  Rt -> Rf [dr.snd=true] / {o=dr.fst, ar=true}; *)
-lemma transition_2_0:
+lemma receiverTransition_2_0[simp]:
   assumes "(snd port_dr)=True"
-    shows "receiverTransition ((ReceiverState Rt ), (receiverElemIn_Dr (Msg port_dr)))
-         = (ReceiverState Rf, (receiverOut_Ar_O (Msg (True)) (Msg ((fst port_dr)))))"
-  oops
+    shows "receiverTransition ((ReceiverState Rt ), (receiverElemIn_dr (Msg port_dr)))
+         = (ReceiverState Rf, (receiverOut_ar_o (Msg (True)) (Msg ((fst port_dr)))))"
+  apply(simp add: receiverTransition_def)
+  sorry
 
 (* Line 15:  Rt -> Rt [dr.snd=false] / {ar=false}; *)
-lemma transition_2_1:
+lemma receiverTransition_2_1[simp]:
   assumes "(snd port_dr)=False"
-    shows "receiverTransition ((ReceiverState Rt ), (receiverElemIn_Dr (Msg port_dr)))
-         = (ReceiverState Rt, (receiverOut_Ar_O (Msg (False)) null))"
-  oops
+    shows "receiverTransition ((ReceiverState Rt ), (receiverElemIn_dr (Msg port_dr)))
+         = (ReceiverState Rt, (receiverOut_ar_o (Msg (False)) null))"
+  apply(simp add: receiverTransition_def)
+  sorry
 
 (* Line 16:  Rt -> Rt {dr==null}; *)
-lemma transition_3_0:
+lemma receiverTransition_3_0[simp]:
   assumes "True"
-    shows "receiverTransition ((ReceiverState Rt ), (receiverElemIn_Dr null))
-         = (ReceiverState Rt, (receiverOut_Ar_O null null))"
-  oops
+    shows "receiverTransition ((ReceiverState Rt ), (receiverElemIn_dr null))
+         = (ReceiverState Rt, (receiverOut_ar_o null null))"
+  apply(simp add: receiverTransition_def)
+  sorry
 
 
 section \<open>Step-wise lemmata for the SPF\<close>
 
-(* SWS: I am moving this to dAutomaton *)
-lemma da_h_stepI: assumes "sbeDom sbe = daDom da"
-  assumes "(daNextOutput da s sbe)  = out"
-      and "(daNextState da s sbe) = nextState"
-  shows "spfConcIn (sbe2SB sbe)\<cdot>(da_h da s) = spfConcOut out\<cdot>((da_h da nextState))"
-  by (metis (no_types) assms da_h_dom da_h_final_h3 spfConcIn_dom spfConcIn_step spfConcOut_dom spf_eq)
-
-
+(* Convert the SPF to step notation *)
+lemma receiverSpf2Step: "receiverSPF = spfConcOut (receiverOut_ar_o null null)\<cdot>(ReceiverStep (ReceiverState Rt ))"
+  sorry
 
 (* Line 18:  Rf -> Rf [dr.snd=true] / {ar=true}; *)
-lemma step_0_0:
+lemma receiverStep_0_0:
   assumes "(snd port_dr)=True"
-    shows "spfConcIn  (receiverIn_Dr (Msg port_dr))\<cdot>(ReceiverStep (ReceiverState Rf ))
-         = spfConcOut (receiverOut_Ar_O (Msg (True)) null)\<cdot>(ReceiverStep (ReceiverState Rf))"
-  apply(simp add: ReceiverStep_def)
+    shows "spfConcIn  (receiverIn_dr (Msg port_dr))\<cdot>(receiverStep (ReceiverState Rf ))
+         = spfConcOut (receiverOut_ar_o (Msg (True)) null)\<cdot>(receiverStep (ReceiverState Rf))"
+  apply(simp add: receiverStep_def receiverIn_dr_def)
   apply(rule da_h_stepI)
-  by(auto simp add: daNextState_def daNextOutput_def assms)
-  (* SWS: Bäm! *)
+  apply(auto simp add: daNextState_def daNextOutput_def assms)
+  (* TODO SWS: Manchmal fehlt noch das hier: *)
+  (*using assms by auto*)
+  sorry
 
 (* Line 19:  Rf -> Rt [dr.snd=false] / {ar=false, o=dr.fst}; *)
-lemma step_0_1:
+lemma receiverStep_0_1:
   assumes "(snd port_dr)=False"
-    shows "spfConcIn  (receiverIn_Dr (Msg port_dr))\<cdot>(ReceiverStep (ReceiverState Rf ))
-         = spfConcOut (receiverOut_Ar_O (Msg (False)) (Msg ((fst port_dr))))\<cdot>(ReceiverStep (ReceiverState Rt))"
-  oops
+    shows "spfConcIn  (receiverIn_dr (Msg port_dr))\<cdot>(receiverStep (ReceiverState Rf ))
+         = spfConcOut (receiverOut_ar_o (Msg (False)) (Msg ((fst port_dr))))\<cdot>(receiverStep (ReceiverState Rt))"
+  apply(simp add: receiverStep_def receiverIn_dr_def)
+  apply(rule da_h_stepI)
+  apply(auto simp add: daNextState_def daNextOutput_def assms)
+  (* TODO SWS: Manchmal fehlt noch das hier: *)
+  (*using assms by auto*)
+  sorry
 
 (* Line 17:  Rf -> Rf {dr==null}; *)
-lemma step_1_0:
+lemma receiverStep_1_0:
   assumes "True"
-    shows "spfConcIn  (receiverIn_Dr null)\<cdot>(ReceiverStep (ReceiverState Rf ))
-         = spfConcOut (receiverOut_Ar_O null null)\<cdot>(ReceiverStep (ReceiverState Rf))"
-  oops
+    shows "spfConcIn  (receiverIn_dr null)\<cdot>(receiverStep (ReceiverState Rf ))
+         = spfConcOut (receiverOut_ar_o null null)\<cdot>(receiverStep (ReceiverState Rf))"
+  apply(simp add: receiverStep_def receiverIn_dr_def)
+  apply(rule da_h_stepI)
+  apply(auto simp add: daNextState_def daNextOutput_def assms)
+  (* TODO SWS: Manchmal fehlt noch das hier: *)
+  (*using assms by auto*)
+  sorry
 
 (* Line 14:  Rt -> Rf [dr.snd=true] / {o=dr.fst, ar=true}; *)
-lemma step_2_0:
+lemma receiverStep_2_0:
   assumes "(snd port_dr)=True"
-    shows "spfConcIn  (receiverIn_Dr (Msg port_dr))\<cdot>(ReceiverStep (ReceiverState Rt ))
-         = spfConcOut (receiverOut_Ar_O (Msg (True)) (Msg ((fst port_dr))))\<cdot>(ReceiverStep (ReceiverState Rf))"
-  oops
+    shows "spfConcIn  (receiverIn_dr (Msg port_dr))\<cdot>(receiverStep (ReceiverState Rt ))
+         = spfConcOut (receiverOut_ar_o (Msg (True)) (Msg ((fst port_dr))))\<cdot>(receiverStep (ReceiverState Rf))"
+  apply(simp add: receiverStep_def receiverIn_dr_def)
+  apply(rule da_h_stepI)
+  apply(auto simp add: daNextState_def daNextOutput_def assms)
+  (* TODO SWS: Manchmal fehlt noch das hier: *)
+  (*using assms by auto*)
+  sorry
 
 (* Line 15:  Rt -> Rt [dr.snd=false] / {ar=false}; *)
-lemma step_2_1:
+lemma receiverStep_2_1:
   assumes "(snd port_dr)=False"
-    shows "spfConcIn  (receiverIn_Dr (Msg port_dr))\<cdot>(ReceiverStep (ReceiverState Rt ))
-         = spfConcOut (receiverOut_Ar_O (Msg (False)) null)\<cdot>(ReceiverStep (ReceiverState Rt))"
-  oops
+    shows "spfConcIn  (receiverIn_dr (Msg port_dr))\<cdot>(receiverStep (ReceiverState Rt ))
+         = spfConcOut (receiverOut_ar_o (Msg (False)) null)\<cdot>(receiverStep (ReceiverState Rt))"
+  apply(simp add: receiverStep_def receiverIn_dr_def)
+  apply(rule da_h_stepI)
+  apply(auto simp add: daNextState_def daNextOutput_def assms)
+  (* TODO SWS: Manchmal fehlt noch das hier: *)
+  (*using assms by auto*)
+  sorry
 
 (* Line 16:  Rt -> Rt {dr==null}; *)
-lemma step_3_0:
+lemma receiverStep_3_0:
   assumes "True"
-    shows "spfConcIn  (receiverIn_Dr null)\<cdot>(ReceiverStep (ReceiverState Rt ))
-         = spfConcOut (receiverOut_Ar_O null null)\<cdot>(ReceiverStep (ReceiverState Rt))"
-  oops
-
-
-
-(* SWS: one more lemma :D *)
-lemma "ReceiverSPF = spfConcOut (receiverOut_Ar_O null null)\<cdot>(ReceiverStep (ReceiverState Rt))"
+    shows "spfConcIn  (receiverIn_dr null)\<cdot>(receiverStep (ReceiverState Rt ))
+         = spfConcOut (receiverOut_ar_o null null)\<cdot>(receiverStep (ReceiverState Rt))"
+  apply(simp add: receiverStep_def receiverIn_dr_def)
+  apply(rule da_h_stepI)
+  apply(auto simp add: daNextState_def daNextOutput_def assms)
+  (* TODO SWS: Manchmal fehlt noch das hier: *)
+  (*using assms by auto*)
   sorry
+
 
 end
