abp/SenderAutomaton.thy
@@ -3,12 +3,24 @@
  * This file was generated from Sender.maa and will be overridden when changed. To change
  * permanently, consider changing the model itself.
  *
- * Generated on Sep 21, 2018 4:47:19 PM by isartransformer 1.0.0
+ * Generated on Sep 22, 2018 1:11:51 PM by isartransformer 1.0.0
  *)
 theory SenderAutomaton
   imports bundle.tsynBundle automat.dAutomaton
 
 begin
+
+
+(* TODO SWS: Move this to dAutomaton *)
+lemma da_h_stepI:
+  assumes "sbeDom sbe = daDom da"
+      and "(daNextOutput da s sbe) = out"
+      and "(daNextState da s sbe) = nextState"
+  shows "spfConcIn (sbe2SB sbe)\<cdot>(da_h da s) = spfConcOut out\<cdot>(da_h da nextState)"
+  by (metis (no_types) assms da_h_dom da_h_final_h3 spfConcIn_dom spfConcIn_step spfConcOut_dom spf_eq)
+
+(* TODO SWS: Move this to...? *)
+setup_lifting type_definition_cfun
 
 (* Helper for easier generation *)
 fun prepend :: "'a::type list \<Rightarrow> 'a \<Rightarrow> 'a list" where
@@ -17,40 +29,41 @@ fun prepend :: "'a::type list \<Rightarrow> 'a \<Rightarrow> 'a list" where
 section \<open>Datatype definition\<close>
 
 datatype senderMessage = SenderBool "bool" | SenderNat "nat" | SenderPair_SenderNat_SenderBool "(nat\<times>bool)"
+
 instance senderMessage :: countable
   apply(intro_classes)
   by(countable_datatype)
 
 instantiation senderMessage :: message
 begin
-  fun ctype_senderMessage :: "channel  \<Rightarrow> senderMessage set" where
+  fun ctype_senderMessage :: "channel \<Rightarrow> senderMessage set" where
   "ctype_senderMessage c = (
     if c = \<C> ''as'' then range SenderBool else
     if c = \<C> ''i'' then range SenderNat else
     if c = \<C> ''ds'' then range SenderPair_SenderNat_SenderBool else
-    {})"
-    instance
+    undefined)"
+  instance
     by(intro_classes)
 end
 
 
 section \<open>Helpers to create a bundle from a single raw element\<close>
 
-lift_definition senderElem_raw_As :: "bool \<Rightarrow> senderMessage tsyn sbElem" is
+lift_definition senderElem_raw_as :: "bool \<Rightarrow> senderMessage tsyn sbElem" is
 "\<lambda>x. [\<C> ''as'' \<mapsto> Msg (SenderBool x)]"
   unfolding sbElemWell_def
   unfolding usclOkay_stream_def
   unfolding ctype_tsyn_def
   by simp
 
-lift_definition senderElem_raw_I :: "nat \<Rightarrow> senderMessage tsyn sbElem" is
+lift_definition senderElem_raw_i :: "nat \<Rightarrow> senderMessage tsyn sbElem" is
 "\<lambda>x. [\<C> ''i'' \<mapsto> Msg (SenderNat x)]"
   unfolding sbElemWell_def
   unfolding usclOkay_stream_def
   unfolding ctype_tsyn_def
   by simp
 
-lift_definition senderElem_raw_Ds :: "(nat\<times>bool) \<Rightarrow> senderMessage tsyn sbElem" is
+lift_definition senderElem_raw_ds :: "(nat\<times>bool) \<Rightarrow> senderMessage tsyn sbElem" is
 "\<lambda>x. [\<C> ''ds'' \<mapsto> Msg (SenderPair_SenderNat_SenderBool x)]"
   unfolding sbElemWell_def
   unfolding usclOkay_stream_def
@@ -60,107 +73,136 @@ lift_definition senderElem_raw_Ds :: "(nat\<times>bool) \<Rightarrow> senderMess
 
 section \<open>Helpers to create a bundle from a single tsyn element\<close>
 
-fun senderElem_As :: "bool tsyn \<Rightarrow> senderMessage tsyn sbElem" where
-"senderElem_As (Msg port_as) = senderElem_raw_As port_as" |
-"senderElem_As null = sbeNull {\<C> ''as''}"
+fun senderElem_as :: "bool tsyn \<Rightarrow> senderMessage tsyn sbElem" where
+"senderElem_as (Msg port_as) = senderElem_raw_as port_as" |
+"senderElem_as null = sbeNull {\<C> ''as''}"
 
-definition sender_As :: "bool tsyn \<Rightarrow> senderMessage tsyn SB" where
-"sender_As port_as = sbe2SB (senderElem_As port_as)"
+declare senderElem_as.simps[simp del]
 
-fun senderElem_I :: "nat tsyn \<Rightarrow> senderMessage tsyn sbElem" where
-"senderElem_I (Msg port_i) = senderElem_raw_I port_i" |
-"senderElem_I null = sbeNull {\<C> ''i''}"
+definition sender_as :: "bool tsyn \<Rightarrow> senderMessage tsyn SB" where
+"sender_as port_as = sbe2SB (senderElem_as port_as)"
 
-definition sender_I :: "nat tsyn \<Rightarrow> senderMessage tsyn SB" where
-"sender_I port_i = sbe2SB (senderElem_I port_i)"
+fun senderElem_i :: "nat tsyn \<Rightarrow> senderMessage tsyn sbElem" where
+"senderElem_i (Msg port_i) = senderElem_raw_i port_i" |
+"senderElem_i null = sbeNull {\<C> ''i''}"
 
-fun senderElem_Ds :: "(nat\<times>bool) tsyn \<Rightarrow> senderMessage tsyn sbElem" where
-"senderElem_Ds (Msg port_ds) = senderElem_raw_Ds port_ds" |
-"senderElem_Ds null = sbeNull {\<C> ''ds''}"
+declare senderElem_i.simps[simp del]
 
-definition sender_Ds :: "(nat\<times>bool) tsyn \<Rightarrow> senderMessage tsyn SB" where
-"sender_Ds port_ds = sbe2SB (senderElem_Ds port_ds)"
+definition sender_i :: "nat tsyn \<Rightarrow> senderMessage tsyn SB" where
+"sender_i port_i = sbe2SB (senderElem_i port_i)"
+
+fun senderElem_ds :: "(nat\<times>bool) tsyn \<Rightarrow> senderMessage tsyn sbElem" where
+"senderElem_ds (Msg port_ds) = senderElem_raw_ds port_ds" |
+"senderElem_ds null = sbeNull {\<C> ''ds''}"
+
+declare senderElem_ds.simps[simp del]
+
+definition sender_ds :: "(nat\<times>bool) tsyn \<Rightarrow> senderMessage tsyn SB" where
+"sender_ds port_ds = sbe2SB (senderElem_ds port_ds)"
 
 (* Create one sbElem for all input channels *)
-fun senderElemIn_As_I :: "bool tsyn \<Rightarrow> nat tsyn \<Rightarrow> senderMessage tsyn sbElem" where
-"senderElemIn_As_I port_as port_i = (senderElem_As port_as) \<plusminus> (senderElem_I port_i)"
+definition senderElemIn_as_i :: "bool tsyn \<Rightarrow> nat tsyn \<Rightarrow> senderMessage tsyn sbElem" where
+"senderElemIn_as_i port_as port_i = (senderElem_as port_as) \<plusminus> (senderElem_i port_i)"
 
 (* Create one sbElem for all output channels *)
-fun senderElemOut_Ds :: "(nat\<times>bool) tsyn \<Rightarrow> senderMessage tsyn sbElem" where
-"senderElemOut_Ds port_ds = (senderElem_Ds port_ds)"
+definition senderElemOut_ds :: "(nat\<times>bool) tsyn \<Rightarrow> senderMessage tsyn sbElem" where
+"senderElemOut_ds port_ds = (senderElem_ds port_ds)"
 
 (* Create one SB for all input channels *)
-fun senderIn_As_I :: "bool tsyn \<Rightarrow> nat tsyn \<Rightarrow> senderMessage tsyn SB" where
-"senderIn_As_I port_as port_i = (sbe2SB (senderElemIn_As_I port_as port_i))"
+definition senderIn_as_i :: "bool tsyn \<Rightarrow> nat tsyn \<Rightarrow> senderMessage tsyn SB" where
+"senderIn_as_i port_as port_i = (sbe2SB (senderElemIn_as_i port_as port_i))"
 
 (* Create one SB for all output channels *)
-fun senderOut_Ds :: "(nat\<times>bool) tsyn \<Rightarrow> senderMessage tsyn SB" where
-"senderOut_Ds port_ds = (sbe2SB (senderElemOut_Ds port_ds))"
+definition senderOut_ds :: "(nat\<times>bool) tsyn \<Rightarrow> senderMessage tsyn SB" where
+"senderOut_ds port_ds = (sbe2SB (senderElemOut_ds port_ds))"
 
 
 section \<open>Helpers to create a bundle from a tsyn list of elements\<close>
 
-fun sender_list_As :: "(bool tsyn) list \<Rightarrow> senderMessage tsyn SB" where
-"sender_list_As (x#xs) = ubConcEq (sender_As x)\<cdot>(sender_list_As xs)" |
-"sender_list_As []     = ubLeast {\<C> ''as''}"
+fun sender_list_as :: "(bool tsyn) list \<Rightarrow> senderMessage tsyn SB" where
+"sender_list_as (x#xs) = ubConcEq (sender_as x)\<cdot>(sender_list_as xs)" |
+"sender_list_as []     = ubLeast {\<C> ''as''}"
 
-fun sender_list_I :: "(nat tsyn) list \<Rightarrow> senderMessage tsyn SB" where
-"sender_list_I (x#xs) = ubConcEq (sender_I x)\<cdot>(sender_list_I xs)" |
-"sender_list_I []     = ubLeast {\<C> ''i''}"
+fun sender_list_i :: "(nat tsyn) list \<Rightarrow> senderMessage tsyn SB" where
+"sender_list_i (x#xs) = ubConcEq (sender_i x)\<cdot>(sender_list_i xs)" |
+"sender_list_i []     = ubLeast {\<C> ''i''}"
 
-fun sender_list_Ds :: "((nat\<times>bool) tsyn) list \<Rightarrow> senderMessage tsyn SB" where
-"sender_list_Ds (x#xs) = ubConcEq (sender_Ds x)\<cdot>(sender_list_Ds xs)" |
-"sender_list_Ds []     = ubLeast {\<C> ''ds''}"
+fun sender_list_ds :: "((nat\<times>bool) tsyn) list \<Rightarrow> senderMessage tsyn SB" where
+"sender_list_ds (x#xs) = ubConcEq (sender_ds x)\<cdot>(sender_list_ds xs)" |
+"sender_list_ds []     = ubLeast {\<C> ''ds''}"
 
 (* Create one SB for all input channels *)
-fun senderIn_list_As_I :: "bool tsyn list \<Rightarrow> nat tsyn list \<Rightarrow> senderMessage tsyn SB" where
-"senderIn_list_As_I port_as port_i = (sender_list_As port_as) \<uplus> (sender_list_I port_i)"
+definition senderIn_list_as_i :: "bool tsyn list \<Rightarrow> nat tsyn list \<Rightarrow> senderMessage tsyn SB" where
+"senderIn_list_as_i port_as port_i = (sender_list_as port_as) \<uplus> (sender_list_i port_i)"
 
 (* Create one SB for all output channels *)
-fun senderOut_list_Ds :: "(nat\<times>bool) tsyn list \<Rightarrow> senderMessage tsyn SB" where
-"senderOut_list_Ds port_ds = (sender_list_Ds port_ds)"
+definition senderOut_list_ds :: "(nat\<times>bool) tsyn list \<Rightarrow> senderMessage tsyn SB" where
+"senderOut_list_ds port_ds = (sender_list_ds port_ds)"
 
 
 section \<open>Helpers to create a bundle from a tsyn stream of elements\<close>
 
-definition sender_stream_As :: "(bool) tsyn stream \<Rightarrow> senderMessage tsyn SB" where
-"sender_stream_As = undefined"
+lift_definition sender_stream_as_h :: "bool tsyn stream \<Rightarrow> senderMessage tsyn SB" is
+"\<lambda> s. [(\<C> ''as'') \<mapsto> (tsynMap (SenderBool)\<cdot>s)]"
+  unfolding ubWell_def usclOkay_stream_def ctype_tsyn_def
+  apply auto
+  sorry
 
-definition sender_stream_I :: "(nat) tsyn stream \<Rightarrow> senderMessage tsyn SB" where
-"sender_stream_I = undefined"
+lift_definition sender_stream_as :: "(bool) tsyn stream \<rightarrow> senderMessage tsyn SB" is
+"sender_stream_as_h"
+  sorry
 
-definition sender_stream_Ds :: "((nat\<times>bool)) tsyn stream \<Rightarrow> senderMessage tsyn SB" where
-"sender_stream_Ds = undefined"
+lift_definition sender_stream_i_h :: "nat tsyn stream \<Rightarrow> senderMessage tsyn SB" is
+"\<lambda> s. [(\<C> ''i'') \<mapsto> (tsynMap (SenderNat)\<cdot>s)]"
+  unfolding ubWell_def usclOkay_stream_def ctype_tsyn_def
+  apply auto
+  sorry
+
+lift_definition sender_stream_i :: "(nat) tsyn stream \<rightarrow> senderMessage tsyn SB" is
+"sender_stream_i_h"
+  sorry
+
+lift_definition sender_stream_ds_h :: "(nat\<times>bool) tsyn stream \<Rightarrow> senderMessage tsyn SB" is
+"\<lambda> s. [(\<C> ''ds'') \<mapsto> (tsynMap (SenderPair_SenderNat_SenderBool)\<cdot>s)]"
+  unfolding ubWell_def usclOkay_stream_def ctype_tsyn_def
+  apply auto
+  sorry
+
+lift_definition sender_stream_ds :: "((nat\<times>bool)) tsyn stream \<rightarrow> senderMessage tsyn SB" is
+"sender_stream_ds_h"
+  sorry
 
 (* Create one SB for all input channels *)
-fun senderIn_stream_As_I :: "bool tsyn stream \<Rightarrow> nat tsyn stream \<Rightarrow> senderMessage tsyn SB" where
-"senderIn_stream_As_I port_as port_i = (sender_stream_As port_as) \<uplus> (sender_stream_I port_i)"
+definition senderIn_stream_as_i :: "bool tsyn stream \<rightarrow> nat tsyn stream \<rightarrow> senderMessage tsyn SB" where
+"senderIn_stream_as_i = (\<Lambda>  port_as port_i. (sender_stream_as\<cdot>port_as) \<uplus> (sender_stream_i\<cdot>port_i))"
 
 (* Create one SB for all output channels *)
-fun senderOut_stream_Ds :: "(nat\<times>bool) tsyn stream \<Rightarrow> senderMessage tsyn SB" where
-"senderOut_stream_Ds port_ds = (sender_stream_Ds port_ds)"
+definition senderOut_stream_ds :: "(nat\<times>bool) tsyn stream \<rightarrow> senderMessage tsyn SB" where
+"senderOut_stream_ds = (\<Lambda>  port_ds. (sender_stream_ds\<cdot>port_ds))"
 
 
 section \<open>Helpers to get tsyn elements and streams from sbElems and SBs\<close>
 
-fun senderElem_get_As :: "senderMessage tsyn sbElem \<Rightarrow> (bool) tsyn" where
-"senderElem_get_As sbe = undefined"
+fun senderElem_get_as :: "senderMessage tsyn sbElem \<Rightarrow> (bool) tsyn" where
+"senderElem_get_as sbe = undefined"
 
-fun senderElem_get_stream_As :: "senderMessage tsyn SB \<Rightarrow> (bool) tsyn stream" where
-"senderElem_get_stream_As sb = undefined"
+lift_definition sender_get_stream_as :: "senderMessage tsyn SB \<rightarrow> bool tsyn stream" is
+"\<lambda>sb. tsynMap (inv SenderBool)\<cdot>(sb . (\<C> ''as''))"
+  by(simp add: cfun_def)
 
-fun senderElem_get_I :: "senderMessage tsyn sbElem \<Rightarrow> (nat) tsyn" where
-"senderElem_get_I sbe = undefined"
+fun senderElem_get_i :: "senderMessage tsyn sbElem \<Rightarrow> (nat) tsyn" where
+"senderElem_get_i sbe = undefined"
 
-fun senderElem_get_stream_I :: "senderMessage tsyn SB \<Rightarrow> (nat) tsyn stream" where
-"senderElem_get_stream_I sb = undefined"
+lift_definition sender_get_stream_i :: "senderMessage tsyn SB \<rightarrow> nat tsyn stream" is
+"\<lambda>sb. tsynMap (inv SenderNat)\<cdot>(sb . (\<C> ''i''))"
+  by(simp add: cfun_def)
 
-fun senderElem_get_Ds :: "senderMessage tsyn sbElem \<Rightarrow> ((nat\<times>bool)) tsyn" where
-"senderElem_get_Ds sbe = undefined"
+fun senderElem_get_ds :: "senderMessage tsyn sbElem \<Rightarrow> ((nat\<times>bool)) tsyn" where
+"senderElem_get_ds sbe = undefined"
 
-fun senderElem_get_stream_Ds :: "senderMessage tsyn SB \<Rightarrow> ((nat\<times>bool)) tsyn stream" where
-"senderElem_get_stream_Ds sb = undefined"
-
+lift_definition sender_get_stream_ds :: "senderMessage tsyn SB \<rightarrow> (nat\<times>bool) tsyn stream" is
+"\<lambda>sb. tsynMap (inv SenderPair_SenderNat_SenderBool)\<cdot>(sb . (\<C> ''ds''))"
+  by(simp add: cfun_def)
 
 
 
@@ -187,60 +229,60 @@ fun getC :: "SenderState \<Rightarrow> nat" where
 (* Helper that allows us to utilize pattern matching *)
 fun senderTransitionH :: "(SenderState \<times> (bool tsyn \<times> nat tsyn)) \<Rightarrow> (SenderState \<times> senderMessage tsyn SB)" where
 "senderTransitionH (SenderState Sf var_buffer var_c, (\<^cancel>\<open>as\<mapsto>\<close>Msg port_as, \<^cancel>\<open>i\<mapsto>\<close>Msg port_i)) =
-  (if((size var_buffer)>1 \<and> port_as=False) then ((SenderState St (prepend (butlast var_buffer) port_i) 3, (senderOut_Ds (Msg (Pair (last (butlast var_buffer)) True)))))
-   else if((size var_buffer)=1 \<and> port_as=False) then ((SenderState St (prepend (butlast var_buffer) port_i) 3, (senderOut_Ds (Msg (Pair port_i True)))))
-   else if((size var_buffer)=0) then ((SenderState Sf (prepend var_buffer port_i) 3, (senderOut_Ds (Msg (Pair port_i False)))))
-   else if((size var_buffer)>0 \<and> var_c>0 \<and> port_as=True) then ((SenderState Sf (prepend var_buffer port_i) (var_c-1), (senderOut_Ds null)))
-   else if((size var_buffer)>0 \<and> var_c=0 \<and> port_as=True) then ((SenderState Sf (prepend var_buffer port_i) 3, (senderOut_Ds (Msg (Pair (last var_buffer) False)))))
-   else (SenderState Sf var_buffer var_c, (senderOut_Ds null)))" |
+  (if((size var_buffer)>1 \<and> port_as=False) then ((SenderState St (prepend (butlast var_buffer) port_i) 3, (senderOut_ds (Msg (Pair (last (butlast var_buffer)) True)))))
+   else if((size var_buffer)=1 \<and> port_as=False) then ((SenderState St (prepend (butlast var_buffer) port_i) 3, (senderOut_ds (Msg (Pair port_i True)))))
+   else if((size var_buffer)=0) then ((SenderState Sf (prepend var_buffer port_i) 3, (senderOut_ds (Msg (Pair port_i False)))))
+   else if((size var_buffer)>0 \<and> var_c>0 \<and> port_as=True) then ((SenderState Sf (prepend var_buffer port_i) (var_c-1), (senderOut_ds null)))
+   else if((size var_buffer)>0 \<and> var_c=0 \<and> port_as=True) then ((SenderState Sf (prepend var_buffer port_i) 3, (senderOut_ds (Msg (Pair (last var_buffer) False)))))
+   else (SenderState Sf var_buffer var_c, (senderOut_ds null)))" |
 
 "senderTransitionH (SenderState Sf var_buffer var_c, (\<^cancel>\<open>as\<mapsto>\<close>Msg port_as, \<^cancel>\<open>i\<mapsto>\<close>null)) =
-  (if((size var_buffer)>1 \<and> port_as=False) then ((SenderState St (butlast var_buffer) 3, (senderOut_Ds (Msg (Pair (last (butlast var_buffer)) True)))))
-   else if((size var_buffer)=1 \<and> port_as=False) then ((SenderState St (butlast var_buffer) var_c, (senderOut_Ds null)))
-   else if((size var_buffer)=0) then ((SenderState Sf var_buffer var_c, (senderOut_Ds null)))
-   else if((size var_buffer)>0 \<and> var_c>0 \<and> port_as=True) then ((SenderState Sf var_buffer (var_c-1), (senderOut_Ds null)))
-   else if((size var_buffer)>0 \<and> var_c=0 \<and> port_as=True) then ((SenderState Sf var_buffer 3, (senderOut_Ds (Msg (Pair (last var_buffer) False)))))
-   else (SenderState Sf var_buffer var_c, (senderOut_Ds null)))" |
+  (if((size var_buffer)>1 \<and> port_as=False) then ((SenderState St (butlast var_buffer) 3, (senderOut_ds (Msg (Pair (last (butlast var_buffer)) True)))))
+   else if((size var_buffer)=1 \<and> port_as=False) then ((SenderState St (butlast var_buffer) var_c, (senderOut_ds null)))
+   else if((size var_buffer)=0) then ((SenderState Sf var_buffer var_c, (senderOut_ds null)))
+   else if((size var_buffer)>0 \<and> var_c>0 \<and> port_as=True) then ((SenderState Sf var_buffer (var_c-1), (senderOut_ds null)))
+   else if((size var_buffer)>0 \<and> var_c=0 \<and> port_as=True) then ((SenderState Sf var_buffer 3, (senderOut_ds (Msg (Pair (last var_buffer) False)))))
+   else (SenderState Sf var_buffer var_c, (senderOut_ds null)))" |
 
 "senderTransitionH (SenderState Sf var_buffer var_c, (\<^cancel>\<open>as\<mapsto>\<close>null, \<^cancel>\<open>i\<mapsto>\<close>Msg port_i)) =
-  (if((size var_buffer)=0) then ((SenderState Sf (prepend var_buffer port_i) 3, (senderOut_Ds (Msg (Pair port_i False)))))
-   else if((size var_buffer)>0 \<and> var_c>0) then ((SenderState Sf (prepend var_buffer port_i) (var_c-1), (senderOut_Ds null)))
-   else if((size var_buffer)>0 \<and> var_c=0) then ((SenderState Sf (prepend var_buffer port_i) 3, (senderOut_Ds (Msg (Pair (last var_buffer) False)))))
-   else (SenderState Sf var_buffer var_c, (senderOut_Ds null)))" |
+  (if((size var_buffer)=0) then ((SenderState Sf (prepend var_buffer port_i) 3, (senderOut_ds (Msg (Pair port_i False)))))
+   else if((size var_buffer)>0 \<and> var_c>0) then ((SenderState Sf (prepend var_buffer port_i) (var_c-1), (senderOut_ds null)))
+   else if((size var_buffer)>0 \<and> var_c=0) then ((SenderState Sf (prepend var_buffer port_i) 3, (senderOut_ds (Msg (Pair (last var_buffer) False)))))
+   else (SenderState Sf var_buffer var_c, (senderOut_ds null)))" |
 
 "senderTransitionH (SenderState Sf var_buffer var_c, (\<^cancel>\<open>as\<mapsto>\<close>null, \<^cancel>\<open>i\<mapsto>\<close>null)) =
-  (if((size var_buffer)=0) then ((SenderState Sf var_buffer var_c, (senderOut_Ds null)))
-   else if((size var_buffer)>0 \<and> var_c>0) then ((SenderState Sf var_buffer var_c, (senderOut_Ds null)))
-   else if((size var_buffer)>0 \<and> var_c=0) then ((SenderState Sf var_buffer 3, (senderOut_Ds (Msg (Pair (last var_buffer) False)))))
-   else (SenderState Sf var_buffer var_c, (senderOut_Ds null)))" |
+  (if((size var_buffer)=0) then ((SenderState Sf var_buffer var_c, (senderOut_ds null)))
+   else if((size var_buffer)>0 \<and> var_c>0) then ((SenderState Sf var_buffer var_c, (senderOut_ds null)))
+   else if((size var_buffer)>0 \<and> var_c=0) then ((SenderState Sf var_buffer 3, (senderOut_ds (Msg (Pair (last var_buffer) False)))))
+   else (SenderState Sf var_buffer var_c, (senderOut_ds null)))" |
 
 "senderTransitionH (SenderState St var_buffer var_c, (\<^cancel>\<open>as\<mapsto>\<close>Msg port_as, \<^cancel>\<open>i\<mapsto>\<close>Msg port_i)) =
-  (if((size var_buffer)=0) then ((SenderState St (prepend var_buffer port_i) 3, (senderOut_Ds (Msg (Pair port_i True)))))
-   else if((size var_buffer)>1 \<and> port_as=True) then ((SenderState Sf (prepend (butlast var_buffer) port_i) 3, (senderOut_Ds (Msg (Pair (last (butlast var_buffer)) False)))))
-   else if((size var_buffer)>0 \<and> var_c>0 \<and> port_as=False) then ((SenderState St (prepend var_buffer port_i) (var_c-1), (senderOut_Ds null)))
-   else if((size var_buffer)>0 \<and> var_c=0 \<and> port_as=False) then ((SenderState St (prepend var_buffer port_i) 3, (senderOut_Ds (Msg (Pair (last var_buffer) True)))))
-   else if((size var_buffer)=1 \<and> port_as=True) then ((SenderState Sf (prepend (butlast var_buffer) port_i) 3, (senderOut_Ds (Msg (Pair port_i False)))))
-   else (SenderState St var_buffer var_c, (senderOut_Ds null)))" |
+  (if((size var_buffer)=0) then ((SenderState St (prepend var_buffer port_i) 3, (senderOut_ds (Msg (Pair port_i True)))))
+   else if((size var_buffer)>1 \<and> port_as=True) then ((SenderState Sf (prepend (butlast var_buffer) port_i) 3, (senderOut_ds (Msg (Pair (last (butlast var_buffer)) False)))))
+   else if((size var_buffer)>0 \<and> var_c>0 \<and> port_as=False) then ((SenderState St (prepend var_buffer port_i) (var_c-1), (senderOut_ds null)))
+   else if((size var_buffer)>0 \<and> var_c=0 \<and> port_as=False) then ((SenderState St (prepend var_buffer port_i) 3, (senderOut_ds (Msg (Pair (last var_buffer) True)))))
+   else if((size var_buffer)=1 \<and> port_as=True) then ((SenderState Sf (prepend (butlast var_buffer) port_i) 3, (senderOut_ds (Msg (Pair port_i False)))))
+   else (SenderState St var_buffer var_c, (senderOut_ds null)))" |
 
 "senderTransitionH (SenderState St var_buffer var_c, (\<^cancel>\<open>as\<mapsto>\<close>Msg port_as, \<^cancel>\<open>i\<mapsto>\<close>null)) =
-  (if((size var_buffer)=0) then ((SenderState St var_buffer var_c, (senderOut_Ds null)))
-   else if((size var_buffer)>1 \<and> port_as=True) then ((SenderState Sf (butlast var_buffer) 3, (senderOut_Ds (Msg (Pair (last (butlast var_buffer)) False)))))
-   else if((size var_buffer)>0 \<and> var_c>0 \<and> port_as=False) then ((SenderState St var_buffer (var_c-1), (senderOut_Ds null)))
-   else if((size var_buffer)>0 \<and> var_c=0 \<and> port_as=False) then ((SenderState St var_buffer 3, (senderOut_Ds (Msg (Pair (last var_buffer) True)))))
-   else if((size var_buffer)=1 \<and> port_as=True) then ((SenderState Sf (butlast var_buffer) var_c, (senderOut_Ds null)))
-   else (SenderState St var_buffer var_c, (senderOut_Ds null)))" |
+  (if((size var_buffer)=0) then ((SenderState St var_buffer var_c, (senderOut_ds null)))
+   else if((size var_buffer)>1 \<and> port_as=True) then ((SenderState Sf (butlast var_buffer) 3, (senderOut_ds (Msg (Pair (last (butlast var_buffer)) False)))))
+   else if((size var_buffer)>0 \<and> var_c>0 \<and> port_as=False) then ((SenderState St var_buffer (var_c-1), (senderOut_ds null)))
+   else if((size var_buffer)>0 \<and> var_c=0 \<and> port_as=False) then ((SenderState St var_buffer 3, (senderOut_ds (Msg (Pair (last var_buffer) True)))))
+   else if((size var_buffer)=1 \<and> port_as=True) then ((SenderState Sf (butlast var_buffer) var_c, (senderOut_ds null)))
+   else (SenderState St var_buffer var_c, (senderOut_ds null)))" |
 
 "senderTransitionH (SenderState St var_buffer var_c, (\<^cancel>\<open>as\<mapsto>\<close>null, \<^cancel>\<open>i\<mapsto>\<close>Msg port_i)) =
-  (if((size var_buffer)=0) then ((SenderState St (prepend var_buffer port_i) 3, (senderOut_Ds (Msg (Pair port_i True)))))
-   else if((size var_buffer)>0 \<and> var_c>0) then ((SenderState St (prepend var_buffer port_i) (var_c-1), (senderOut_Ds null)))
-   else if((size var_buffer)>0 \<and> var_c=0) then ((SenderState St (prepend var_buffer port_i) 3, (senderOut_Ds (Msg (Pair (last var_buffer) True)))))
-   else (SenderState St var_buffer var_c, (senderOut_Ds null)))" |
+  (if((size var_buffer)=0) then ((SenderState St (prepend var_buffer port_i) 3, (senderOut_ds (Msg (Pair port_i True)))))
+   else if((size var_buffer)>0 \<and> var_c>0) then ((SenderState St (prepend var_buffer port_i) (var_c-1), (senderOut_ds null)))
+   else if((size var_buffer)>0 \<and> var_c=0) then ((SenderState St (prepend var_buffer port_i) 3, (senderOut_ds (Msg (Pair (last var_buffer) True)))))
+   else (SenderState St var_buffer var_c, (senderOut_ds null)))" |
 
 "senderTransitionH (SenderState St var_buffer var_c, (\<^cancel>\<open>as\<mapsto>\<close>null, \<^cancel>\<open>i\<mapsto>\<close>null)) =
-  (if((size var_buffer)=0) then ((SenderState St var_buffer var_c, (senderOut_Ds null)))
-   else if((size var_buffer)>0 \<and> var_c>0) then ((SenderState St var_buffer (var_c-1), (senderOut_Ds null)))
-   else if((size var_buffer)>0 \<and> var_c=0) then ((SenderState St var_buffer 3, (senderOut_Ds (Msg (Pair (last var_buffer) True)))))
-   else (SenderState St var_buffer var_c, (senderOut_Ds null)))"
+  (if((size var_buffer)=0) then ((SenderState St var_buffer var_c, (senderOut_ds null)))
+   else if((size var_buffer)>0 \<and> var_c>0) then ((SenderState St var_buffer (var_c-1), (senderOut_ds null)))
+   else if((size var_buffer)>0 \<and> var_c=0) then ((SenderState St var_buffer 3, (senderOut_ds (Msg (Pair (last var_buffer) True)))))
+   else (SenderState St var_buffer var_c, (senderOut_ds null)))"
 
 (* Domain *)
 definition senderDom :: "channel set" where
@@ -251,475 +293,733 @@ definition senderRan :: "channel set" where
 "senderRan = {\<C> ''ds''}"
 
 (* Transition function *)
-fun senderTransition :: "(SenderState \<times> senderMessage tsyn sbElem) \<Rightarrow> (SenderState \<times> senderMessage tsyn SB)" where
-"senderTransition (s,b) = (if (sbeDom b) = senderDom then senderTransitionH (s, (senderElem_get_As b, senderElem_get_I b)) else undefined)"
+definition senderTransition :: "(SenderState \<times> senderMessage tsyn sbElem) \<Rightarrow> (SenderState \<times> senderMessage tsyn SB)" where
+"senderTransition = (\<lambda> (s,b). (if (sbeDom b) = senderDom then senderTransitionH (s, (senderElem_get_as b, senderElem_get_i b)) else undefined))"
+
+(* Initial state *)
+definition senderInitialState :: "SenderState" where
+"senderInitialState = SenderState St []  0"
+
+(* Initial output *)
+definition senderInitialOutput :: "senderMessage tsyn SB" where
+"senderInitialOutput = senderOut_ds null"
 
 (* The final automaton *)
-lift_definition SenderAutomaton :: "(SenderState, senderMessage tsyn) dAutomaton" is
-"(senderTransition, SenderState St []  0, (senderOut_Ds null), senderDom, senderRan)"
+lift_definition senderAutomaton :: "(SenderState, senderMessage tsyn) dAutomaton" is
+"(senderTransition, senderInitialState, senderInitialOutput, senderDom, senderRan)"
   by (simp add: senderDom_def senderRan_def)
 
 (* Stream processing function for each state (handy for step lemmata) *)
-definition SenderStep :: "(SenderState \<Rightarrow> (senderMessage tsyn, senderMessage tsyn) SPF)" where
-"SenderStep = da_h SenderAutomaton"
+definition senderStep :: "(SenderState \<Rightarrow> (senderMessage tsyn, senderMessage tsyn) SPF)" where
+"senderStep = da_h senderAutomaton"
 
 (* The final SPF *)
-definition SenderSPF :: "(senderMessage tsyn, senderMessage tsyn) SPF" where
-"SenderSPF = da_H SenderAutomaton"
+definition senderSPF :: "(senderMessage tsyn, senderMessage tsyn) SPF" where
+"senderSPF = da_H senderAutomaton"
+
+
+section \<open>Lemmas for automaton definition\<close>
+
+lemma senderautomaton_trans[simp]: "daTransition senderAutomaton = senderTransition"
+  sorry
+
+lemma senderautomaton_initialstate[simp]: "daInitialState senderAutomaton = senderInitialState"
+  sorry
+
+lemma senderautomaton_initialoutput[simp]: "daInitialOutput senderAutomaton = senderInitialOutput"
+  sorry
+
+lemma senderautomaton_dom[simp]: "daDom senderAutomaton = senderDom"
+  sorry
+
+lemma senderautomaton_ran[simp]: "daRan senderAutomaton = senderRan"
+  sorry
+
+
+section \<open>Lemmas for single tsyn setter\<close>
+
+lemma senderelemin_as_i_dom[simp]: "sbeDom (senderElemIn_as_i port_as port_i) = senderDom"
+  sorry
+
+lemma senderelemout_ds_dom[simp]: "sbeDom (senderElemOut_ds port_ds) = senderRan"
+  sorry
+
+lemma senderin_as_i_dom[simp]: "ubDom\<cdot>(senderIn_as_i port_as port_i) = senderDom"
+  sorry
+
+lemma senderout_ds_dom[simp]: "ubDom\<cdot>(senderOut_ds port_ds) = senderRan"
+  sorry
+
+
+section \<open>Lemmas for getter\<close>
+
+lemma senderelem_as_id[simp]: "senderElem_get_as (senderElem_as port_as) = port_as"
+  sorry
+
+lemma sender_stream_as_id[simp]: "sender_get_stream_as\<cdot>(sender_stream_as\<cdot>port_as) = port_as"
+  sorry
+
+lemma senderelem_i_id[simp]: "senderElem_get_i (senderElem_i port_i) = port_i"
+  sorry
+
+lemma sender_stream_i_id[simp]: "sender_get_stream_i\<cdot>(sender_stream_i\<cdot>port_i) = port_i"
+  sorry
+
+lemma senderelem_ds_id[simp]: "senderElem_get_ds (senderElem_ds port_ds) = port_ds"
+  sorry
+
+lemma sender_stream_ds_id[simp]: "sender_get_stream_ds\<cdot>(sender_stream_ds\<cdot>port_ds) = port_ds"
+  sorry
 
 
 section \<open>Step-wise lemmata for the transition function\<close>
 
 (* Line 33:  Sf -> St [buffer.size()>1 && i!=null] {as==false} / {buffer=buffer.butlast().prepend(i), c=3, ds=new Pair<>(buffer.butlast().last(),true)}; *)
-lemma transition_0_0:
+lemma senderTransition_0_0[simp]:
   assumes "(size var_buffer)>1 \<and> port_as=False"
-    shows "senderTransition ((SenderState Sf var_buffer var_c), (senderElemIn_As_I (Msg port_as) (Msg port_i)))
-         = (SenderState St (prepend (butlast var_buffer) port_i) 3, (senderOut_Ds (Msg (Pair (last (butlast var_buffer)) True))))"
-  oops
+    shows "senderTransition ((SenderState Sf var_buffer var_c), (senderElemIn_as_i (Msg port_as) (Msg port_i)))
+         = (SenderState St (prepend (butlast var_buffer) port_i) 3, (senderOut_ds (Msg (Pair (last (butlast var_buffer)) True))))"
+  apply(simp add: senderTransition_def)
+  sorry
 
 (* Line 35:  Sf -> St [buffer.size()=1 && i!=null] {as==false} / {buffer=buffer.butlast().prepend(i), c=3, ds=new Pair<>(i,true)}; *)
-lemma transition_0_1:
+lemma senderTransition_0_1[simp]:
   assumes "(size var_buffer)=1 \<and> port_as=False"
-    shows "senderTransition ((SenderState Sf var_buffer var_c), (senderElemIn_As_I (Msg port_as) (Msg port_i)))
-         = (SenderState St (prepend (butlast var_buffer) port_i) 3, (senderOut_Ds (Msg (Pair port_i True))))"
-  oops
+    shows "senderTransition ((SenderState Sf var_buffer var_c), (senderElemIn_as_i (Msg port_as) (Msg port_i)))
+         = (SenderState St (prepend (butlast var_buffer) port_i) 3, (senderOut_ds (Msg (Pair port_i True))))"
+  apply(simp add: senderTransition_def)
+  sorry
 
 (* Line 43:  Sf -> Sf [buffer.size()=0 && as!=null && i!=null] / {buffer=buffer.prepend(i), c=3, ds=new Pair<>(i,false)}; *)
-lemma transition_0_2:
+lemma senderTransition_0_2[simp]:
   assumes "(size var_buffer)=0"
-    shows "senderTransition ((SenderState Sf var_buffer var_c), (senderElemIn_As_I (Msg port_as) (Msg port_i)))
-         = (SenderState Sf (prepend var_buffer port_i) 3, (senderOut_Ds (Msg (Pair port_i False))))"
-  oops
+    shows "senderTransition ((SenderState Sf var_buffer var_c), (senderElemIn_as_i (Msg port_as) (Msg port_i)))
+         = (SenderState Sf (prepend var_buffer port_i) 3, (senderOut_ds (Msg (Pair port_i False))))"
+  apply(simp add: senderTransition_def)
+  sorry
 
 (* Line 45:  Sf -> Sf [buffer.size()>0 && c>0 && i!=null] {as==true} / {buffer=buffer.prepend(i), c=c-1}; *)
-lemma transition_0_3:
+lemma senderTransition_0_3[simp]:
   assumes "(size var_buffer)>0 \<and> var_c>0 \<and> port_as=True"
-    shows "senderTransition ((SenderState Sf var_buffer var_c), (senderElemIn_As_I (Msg port_as) (Msg port_i)))
-         = (SenderState Sf (prepend var_buffer port_i) (var_c-1), (senderOut_Ds null))"
-  oops
+    shows "senderTransition ((SenderState Sf var_buffer var_c), (senderElemIn_as_i (Msg port_as) (Msg port_i)))
+         = (SenderState Sf (prepend var_buffer port_i) (var_c-1), (senderOut_ds null))"
+  apply(simp add: senderTransition_def)
+  sorry
 
 (* Line 47:  Sf -> Sf [buffer.size()>0 && c=0 && i!=null] {as==true} / {buffer=buffer.prepend(i), c=3, ds=new Pair<>(buffer.last(),false)}; *)
-lemma transition_0_4:
+lemma senderTransition_0_4[simp]:
   assumes "(size var_buffer)>0 \<and> var_c=0 \<and> port_as=True"
-    shows "senderTransition ((SenderState Sf var_buffer var_c), (senderElemIn_As_I (Msg port_as) (Msg port_i)))
-         = (SenderState Sf (prepend var_buffer port_i) 3, (senderOut_Ds (Msg (Pair (last var_buffer) False))))"
-  oops
+    shows "senderTransition ((SenderState Sf var_buffer var_c), (senderElemIn_as_i (Msg port_as) (Msg port_i)))
+         = (SenderState Sf (prepend var_buffer port_i) 3, (senderOut_ds (Msg (Pair (last var_buffer) False))))"
+  apply(simp add: senderTransition_def)
+  sorry
 
 (* Line 34:  Sf -> St [buffer.size()>1] {as==false, i==null} / {buffer=buffer.butlast(), c=3, ds=new Pair<>(buffer.butlast().last(),true)}; *)
-lemma transition_1_0:
+lemma senderTransition_1_0[simp]:
   assumes "(size var_buffer)>1 \<and> port_as=False"
-    shows "senderTransition ((SenderState Sf var_buffer var_c), (senderElemIn_As_I (Msg port_as) null))
-         = (SenderState St (butlast var_buffer) 3, (senderOut_Ds (Msg (Pair (last (butlast var_buffer)) True))))"
-  oops
+    shows "senderTransition ((SenderState Sf var_buffer var_c), (senderElemIn_as_i (Msg port_as) null))
+         = (SenderState St (butlast var_buffer) 3, (senderOut_ds (Msg (Pair (last (butlast var_buffer)) True))))"
+  apply(simp add: senderTransition_def)
+  sorry
 
 (* Line 36:  Sf -> St [buffer.size()=1] {as==false, i==null} / {buffer=buffer.butlast()}; *)
-lemma transition_1_1:
+lemma senderTransition_1_1[simp]:
   assumes "(size var_buffer)=1 \<and> port_as=False"
-    shows "senderTransition ((SenderState Sf var_buffer var_c), (senderElemIn_As_I (Msg port_as) null))
-         = (SenderState St (butlast var_buffer) var_c, (senderOut_Ds null))"
-  oops
+    shows "senderTransition ((SenderState Sf var_buffer var_c), (senderElemIn_as_i (Msg port_as) null))
+         = (SenderState St (butlast var_buffer) var_c, (senderOut_ds null))"
+  apply(simp add: senderTransition_def)
+  sorry
 
 (* Line 38:  Sf -> Sf [buffer.size()=0 && as!=null] {i==null}; *)
-lemma transition_1_2:
+lemma senderTransition_1_2[simp]:
   assumes "(size var_buffer)=0"
-    shows "senderTransition ((SenderState Sf var_buffer var_c), (senderElemIn_As_I (Msg port_as) null))
-         = (SenderState Sf var_buffer var_c, (senderOut_Ds null))"
-  oops
+    shows "senderTransition ((SenderState Sf var_buffer var_c), (senderElemIn_as_i (Msg port_as) null))
+         = (SenderState Sf var_buffer var_c, (senderOut_ds null))"
+  apply(simp add: senderTransition_def)
+  sorry
 
 (* Line 40:  Sf -> Sf [buffer.size()>0 && c>0] {as==true, i==null} / {c=c-1}; *)
-lemma transition_1_3:
+lemma senderTransition_1_3[simp]:
   assumes "(size var_buffer)>0 \<and> var_c>0 \<and> port_as=True"
-    shows "senderTransition ((SenderState Sf var_buffer var_c), (senderElemIn_As_I (Msg port_as) null))
-         = (SenderState Sf var_buffer (var_c-1), (senderOut_Ds null))"
-  oops
+    shows "senderTransition ((SenderState Sf var_buffer var_c), (senderElemIn_as_i (Msg port_as) null))
+         = (SenderState Sf var_buffer (var_c-1), (senderOut_ds null))"
+  apply(simp add: senderTransition_def)
+  sorry
 
 (* Line 41:  Sf -> Sf [buffer.size()>0 && c=0] {as==true, i==null} / {c=3, ds=new Pair<>(buffer.last(),false)}; *)
-lemma transition_1_4:
+lemma senderTransition_1_4[simp]:
   assumes "(size var_buffer)>0 \<and> var_c=0 \<and> port_as=True"
-    shows "senderTransition ((SenderState Sf var_buffer var_c), (senderElemIn_As_I (Msg port_as) null))
-         = (SenderState Sf var_buffer 3, (senderOut_Ds (Msg (Pair (last var_buffer) False))))"
-  oops
+    shows "senderTransition ((SenderState Sf var_buffer var_c), (senderElemIn_as_i (Msg port_as) null))
+         = (SenderState Sf var_buffer 3, (senderOut_ds (Msg (Pair (last var_buffer) False))))"
+  apply(simp add: senderTransition_def)
+  sorry
 
 (* Line 44:  Sf -> Sf [buffer.size()=0 && i!=null] {as==null} / {buffer=buffer.prepend(i), c=3, ds=new Pair<>(i,false)}; *)
-lemma transition_2_0:
+lemma senderTransition_2_0[simp]:
   assumes "(size var_buffer)=0"
-    shows "senderTransition ((SenderState Sf var_buffer var_c), (senderElemIn_As_I null (Msg port_i)))
-         = (SenderState Sf (prepend var_buffer port_i) 3, (senderOut_Ds (Msg (Pair port_i False))))"
-  oops
+    shows "senderTransition ((SenderState Sf var_buffer var_c), (senderElemIn_as_i null (Msg port_i)))
+         = (SenderState Sf (prepend var_buffer port_i) 3, (senderOut_ds (Msg (Pair port_i False))))"
+  apply(simp add: senderTransition_def)
+  sorry
 
 (* Line 46:  Sf -> Sf [buffer.size()>0 && c>0 && i!=null] {as==null} / {buffer=buffer.prepend(i), c=c-1}; *)
-lemma transition_2_1:
+lemma senderTransition_2_1[simp]:
   assumes "(size var_buffer)>0 \<and> var_c>0"
-    shows "senderTransition ((SenderState Sf var_buffer var_c), (senderElemIn_As_I null (Msg port_i)))
-         = (SenderState Sf (prepend var_buffer port_i) (var_c-1), (senderOut_Ds null))"
-  oops
+    shows "senderTransition ((SenderState Sf var_buffer var_c), (senderElemIn_as_i null (Msg port_i)))
+         = (SenderState Sf (prepend var_buffer port_i) (var_c-1), (senderOut_ds null))"
+  apply(simp add: senderTransition_def)
+  sorry
 
 (* Line 48:  Sf -> Sf [buffer.size()>0 && c=0 && i!=null] {as==null} / {buffer=buffer.prepend(i), c=3, ds=new Pair<>(buffer.last(),false)}; *)
-lemma transition_2_2:
+lemma senderTransition_2_2[simp]:
   assumes "(size var_buffer)>0 \<and> var_c=0"
-    shows "senderTransition ((SenderState Sf var_buffer var_c), (senderElemIn_As_I null (Msg port_i)))
-         = (SenderState Sf (prepend var_buffer port_i) 3, (senderOut_Ds (Msg (Pair (last var_buffer) False))))"
-  oops
+    shows "senderTransition ((SenderState Sf var_buffer var_c), (senderElemIn_as_i null (Msg port_i)))
+         = (SenderState Sf (prepend var_buffer port_i) 3, (senderOut_ds (Msg (Pair (last var_buffer) False))))"
+  apply(simp add: senderTransition_def)
+  sorry
 
 (* Line 37:  Sf -> Sf [buffer.size()=0] {as==null, i==null}; *)
-lemma transition_3_0:
+lemma senderTransition_3_0[simp]:
   assumes "(size var_buffer)=0"
-    shows "senderTransition ((SenderState Sf var_buffer var_c), (senderElemIn_As_I null null))
-         = (SenderState Sf var_buffer var_c, (senderOut_Ds null))"
-  oops
+    shows "senderTransition ((SenderState Sf var_buffer var_c), (senderElemIn_as_i null null))
+         = (SenderState Sf var_buffer var_c, (senderOut_ds null))"
+  apply(simp add: senderTransition_def)
+  sorry
 
 (* Line 39:  Sf -> Sf [buffer.size()>0 && c>0] {as==null, i==null}; *)
-lemma transition_3_1:
+lemma senderTransition_3_1[simp]:
   assumes "(size var_buffer)>0 \<and> var_c>0"
-    shows "senderTransition ((SenderState Sf var_buffer var_c), (senderElemIn_As_I null null))
-         = (SenderState Sf var_buffer var_c, (senderOut_Ds null))"
-  oops
+    shows "senderTransition ((SenderState Sf var_buffer var_c), (senderElemIn_as_i null null))
+         = (SenderState Sf var_buffer var_c, (senderOut_ds null))"
+  apply(simp add: senderTransition_def)
+  sorry
 
 (* Line 42:  Sf -> Sf [buffer.size()>0 && c=0] {as==null, i==null} / {c=3, ds=new Pair<>(buffer.last(),false)}; *)
-lemma transition_3_2:
+lemma senderTransition_3_2[simp]:
   assumes "(size var_buffer)>0 \<and> var_c=0"
-    shows "senderTransition ((SenderState Sf var_buffer var_c), (senderElemIn_As_I null null))
-         = (SenderState Sf var_buffer 3, (senderOut_Ds (Msg (Pair (last var_buffer) False))))"
-  oops
+    shows "senderTransition ((SenderState Sf var_buffer var_c), (senderElemIn_as_i null null))
+         = (SenderState Sf var_buffer 3, (senderOut_ds (Msg (Pair (last var_buffer) False))))"
+  apply(simp add: senderTransition_def)
+  sorry
 
 (* Line 25:  St -> St [buffer.size()=0 && as!=null && i!=null] / {buffer=buffer.prepend(i), c=3, ds=new Pair<>(i,true)}; *)
-lemma transition_4_0:
+lemma senderTransition_4_0[simp]:
   assumes "(size var_buffer)=0"
-    shows "senderTransition ((SenderState St var_buffer var_c), (senderElemIn_As_I (Msg port_as) (Msg port_i)))
-         = (SenderState St (prepend var_buffer port_i) 3, (senderOut_Ds (Msg (Pair port_i True))))"
-  oops
+    shows "senderTransition ((SenderState St var_buffer var_c), (senderElemIn_as_i (Msg port_as) (Msg port_i)))
+         = (SenderState St (prepend var_buffer port_i) 3, (senderOut_ds (Msg (Pair port_i True))))"
+  apply(simp add: senderTransition_def)
+  sorry
 
 (* Line 27:  St -> Sf [buffer.size()>1 && i!=null] {as==true} / {buffer=buffer.butlast().prepend(i), c=3, ds=new Pair<>(buffer.butlast().last(),false)}; *)
-lemma transition_4_1:
+lemma senderTransition_4_1[simp]:
   assumes "(size var_buffer)>1 \<and> port_as=True"
-    shows "senderTransition ((SenderState St var_buffer var_c), (senderElemIn_As_I (Msg port_as) (Msg port_i)))
-         = (SenderState Sf (prepend (butlast var_buffer) port_i) 3, (senderOut_Ds (Msg (Pair (last (butlast var_buffer)) False))))"
-  oops
+    shows "senderTransition ((SenderState St var_buffer var_c), (senderElemIn_as_i (Msg port_as) (Msg port_i)))
+         = (SenderState Sf (prepend (butlast var_buffer) port_i) 3, (senderOut_ds (Msg (Pair (last (butlast var_buffer)) False))))"
+  apply(simp add: senderTransition_def)
+  sorry
 
 (* Line 28:  St -> St [buffer.size()>0 && c>0 && i!=null] {as==false} / {buffer=buffer.prepend(i), c=c-1}; *)
-lemma transition_4_2:
+lemma senderTransition_4_2[simp]:
   assumes "(size var_buffer)>0 \<and> var_c>0 \<and> port_as=False"
-    shows "senderTransition ((SenderState St var_buffer var_c), (senderElemIn_As_I (Msg port_as) (Msg port_i)))
-         = (SenderState St (prepend var_buffer port_i) (var_c-1), (senderOut_Ds null))"
-  oops
+    shows "senderTransition ((SenderState St var_buffer var_c), (senderElemIn_as_i (Msg port_as) (Msg port_i)))
+         = (SenderState St (prepend var_buffer port_i) (var_c-1), (senderOut_ds null))"
+  apply(simp add: senderTransition_def)
+  sorry
 
 (* Line 30:  St -> St [buffer.size()>0 && c=0 && i!=null] {as==false} / {buffer=buffer.prepend(i), c=3, ds=new Pair<>(buffer.last(),true)}; *)
-lemma transition_4_3:
+lemma senderTransition_4_3[simp]:
   assumes "(size var_buffer)>0 \<and> var_c=0 \<and> port_as=False"
-    shows "senderTransition ((SenderState St var_buffer var_c), (senderElemIn_As_I (Msg port_as) (Msg port_i)))
-         = (SenderState St (prepend var_buffer port_i) 3, (senderOut_Ds (Msg (Pair (last var_buffer) True))))"
-  oops
+    shows "senderTransition ((SenderState St var_buffer var_c), (senderElemIn_as_i (Msg port_as) (Msg port_i)))
+         = (SenderState St (prepend var_buffer port_i) 3, (senderOut_ds (Msg (Pair (last var_buffer) True))))"
+  apply(simp add: senderTransition_def)
+  sorry
 
 (* Line 32:  St -> Sf [buffer.size()=1 && i!=null] {as==true} / {buffer=buffer.butlast().prepend(i), c=3, ds=new Pair<>(i,false)}; *)
-lemma transition_4_4:
+lemma senderTransition_4_4[simp]:
   assumes "(size var_buffer)=1 \<and> port_as=True"
-    shows "senderTransition ((SenderState St var_buffer var_c), (senderElemIn_As_I (Msg port_as) (Msg port_i)))
-         = (SenderState Sf (prepend (butlast var_buffer) port_i) 3, (senderOut_Ds (Msg (Pair port_i False))))"
-  oops
+    shows "senderTransition ((SenderState St var_buffer var_c), (senderElemIn_as_i (Msg port_as) (Msg port_i)))
+         = (SenderState Sf (prepend (butlast var_buffer) port_i) 3, (senderOut_ds (Msg (Pair port_i False))))"
+  apply(simp add: senderTransition_def)
+  sorry
 
 (* Line 17:  St -> St [buffer.size()=0 && as!=null] {i==null}; *)
-lemma transition_5_0:
+lemma senderTransition_5_0[simp]:
   assumes "(size var_buffer)=0"
-    shows "senderTransition ((SenderState St var_buffer var_c), (senderElemIn_As_I (Msg port_as) null))
-         = (SenderState St var_buffer var_c, (senderOut_Ds null))"
-  oops
+    shows "senderTransition ((SenderState St var_buffer var_c), (senderElemIn_as_i (Msg port_as) null))
+         = (SenderState St var_buffer var_c, (senderOut_ds null))"
+  apply(simp add: senderTransition_def)
+  sorry
 
 (* Line 18:  St -> Sf [buffer.size()>1] {as==true, i==null} / {buffer=buffer.butlast(), c=3, ds=new Pair<>(buffer.butlast().last(),false)}; *)
-lemma transition_5_1:
+lemma senderTransition_5_1[simp]:
   assumes "(size var_buffer)>1 \<and> port_as=True"
-    shows "senderTransition ((SenderState St var_buffer var_c), (senderElemIn_As_I (Msg port_as) null))
-         = (SenderState Sf (butlast var_buffer) 3, (senderOut_Ds (Msg (Pair (last (butlast var_buffer)) False))))"
-  oops
+    shows "senderTransition ((SenderState St var_buffer var_c), (senderElemIn_as_i (Msg port_as) null))
+         = (SenderState Sf (butlast var_buffer) 3, (senderOut_ds (Msg (Pair (last (butlast var_buffer)) False))))"
+  apply(simp add: senderTransition_def)
+  sorry
 
 (* Line 20:  St -> St [buffer.size()>0 && c>0] {as==false, i==null} / {c=c-1}; *)
-lemma transition_5_2:
+lemma senderTransition_5_2[simp]:
   assumes "(size var_buffer)>0 \<and> var_c>0 \<and> port_as=False"
-    shows "senderTransition ((SenderState St var_buffer var_c), (senderElemIn_As_I (Msg port_as) null))
-         = (SenderState St var_buffer (var_c-1), (senderOut_Ds null))"
-  oops
+    shows "senderTransition ((SenderState St var_buffer var_c), (senderElemIn_as_i (Msg port_as) null))
+         = (SenderState St var_buffer (var_c-1), (senderOut_ds null))"
+  apply(simp add: senderTransition_def)
+  sorry
 
 (* Line 22:  St -> St [buffer.size()>0 && c=0] {as==false, i==null} / {c=3, ds=new Pair<>(buffer.last(),true)}; *)
-lemma transition_5_3:
+lemma senderTransition_5_3[simp]:
   assumes "(size var_buffer)>0 \<and> var_c=0 \<and> port_as=False"
-    shows "senderTransition ((SenderState St var_buffer var_c), (senderElemIn_As_I (Msg port_as) null))
-         = (SenderState St var_buffer 3, (senderOut_Ds (Msg (Pair (last var_buffer) True))))"
-  oops
+    shows "senderTransition ((SenderState St var_buffer var_c), (senderElemIn_as_i (Msg port_as) null))
+         = (SenderState St var_buffer 3, (senderOut_ds (Msg (Pair (last var_buffer) True))))"
+  apply(simp add: senderTransition_def)
+  sorry
 
 (* Line 24:  St -> Sf [buffer.size()=1] {as==true, i==null} / {buffer=buffer.butlast()}; *)
-lemma transition_5_4:
+lemma senderTransition_5_4[simp]:
   assumes "(size var_buffer)=1 \<and> port_as=True"
-    shows "senderTransition ((SenderState St var_buffer var_c), (senderElemIn_As_I (Msg port_as) null))
-         = (SenderState Sf (butlast var_buffer) var_c, (senderOut_Ds null))"
-  oops
+    shows "senderTransition ((SenderState St var_buffer var_c), (senderElemIn_as_i (Msg port_as) null))
+         = (SenderState Sf (butlast var_buffer) var_c, (senderOut_ds null))"
+  apply(simp add: senderTransition_def)
+  sorry
 
 (* Line 26:  St -> St [buffer.size()=0 && i!=null] {as==null} / {buffer=buffer.prepend(i), c=3, ds=new Pair<>(i,true)}; *)
-lemma transition_6_0:
+lemma senderTransition_6_0[simp]:
   assumes "(size var_buffer)=0"
-    shows "senderTransition ((SenderState St var_buffer var_c), (senderElemIn_As_I null (Msg port_i)))
-         = (SenderState St (prepend var_buffer port_i) 3, (senderOut_Ds (Msg (Pair port_i True))))"
-  oops
+    shows "senderTransition ((SenderState St var_buffer var_c), (senderElemIn_as_i null (Msg port_i)))
+         = (SenderState St (prepend var_buffer port_i) 3, (senderOut_ds (Msg (Pair port_i True))))"
+  apply(simp add: senderTransition_def)
+  sorry
 
 (* Line 29:  St -> St [buffer.size()>0 && c>0 && i!=null] {as==null} / {buffer=buffer.prepend(i), c=c-1}; *)
-lemma transition_6_1:
+lemma senderTransition_6_1[simp]:
   assumes "(size var_buffer)>0 \<and> var_c>0"
-    shows "senderTransition ((SenderState St var_buffer var_c), (senderElemIn_As_I null (Msg port_i)))
-         = (SenderState St (prepend var_buffer port_i) (var_c-1), (senderOut_Ds null))"
-  oops
+    shows "senderTransition ((SenderState St var_buffer var_c), (senderElemIn_as_i null (Msg port_i)))
+         = (SenderState St (prepend var_buffer port_i) (var_c-1), (senderOut_ds null))"
+  apply(simp add: senderTransition_def)
+  sorry
 
 (* Line 31:  St -> St [buffer.size()>0 && c=0 && i!=null] {as==null} / {buffer=buffer.prepend(i), c=3, ds=new Pair<>(buffer.last(),true)}; *)
-lemma transition_6_2:
+lemma senderTransition_6_2[simp]:
   assumes "(size var_buffer)>0 \<and> var_c=0"
-    shows "senderTransition ((SenderState St var_buffer var_c), (senderElemIn_As_I null (Msg port_i)))
-         = (SenderState St (prepend var_buffer port_i) 3, (senderOut_Ds (Msg (Pair (last var_buffer) True))))"
-  oops
+    shows "senderTransition ((SenderState St var_buffer var_c), (senderElemIn_as_i null (Msg port_i)))
+         = (SenderState St (prepend var_buffer port_i) 3, (senderOut_ds (Msg (Pair (last var_buffer) True))))"
+  apply(simp add: senderTransition_def)
+  sorry
 
 (* Line 19:  St -> St [buffer.size()=0] {as==null, i==null}; *)
-lemma transition_7_0:
+lemma senderTransition_7_0[simp]:
   assumes "(size var_buffer)=0"
-    shows "senderTransition ((SenderState St var_buffer var_c), (senderElemIn_As_I null null))
-         = (SenderState St var_buffer var_c, (senderOut_Ds null))"
-  oops
+    shows "senderTransition ((SenderState St var_buffer var_c), (senderElemIn_as_i null null))
+         = (SenderState St var_buffer var_c, (senderOut_ds null))"
+  apply(simp add: senderTransition_def)
+  sorry
 
 (* Line 21:  St -> St [buffer.size()>0 && c>0] {as==null, i==null} / {c=c-1}; *)
-lemma transition_7_1:
+lemma senderTransition_7_1[simp]:
   assumes "(size var_buffer)>0 \<and> var_c>0"
-    shows "senderTransition ((SenderState St var_buffer var_c), (senderElemIn_As_I null null))
-         = (SenderState St var_buffer (var_c-1), (senderOut_Ds null))"
-  oops
+    shows "senderTransition ((SenderState St var_buffer var_c), (senderElemIn_as_i null null))
+         = (SenderState St var_buffer (var_c-1), (senderOut_ds null))"
+  apply(simp add: senderTransition_def)
+  sorry
 
 (* Line 23:  St -> St [buffer.size()>0 && c=0] {as==null, i==null} / {c=3, ds=new Pair<>(buffer.last(),true)}; *)
-lemma transition_7_2:
+lemma senderTransition_7_2[simp]:
   assumes "(size var_buffer)>0 \<and> var_c=0"
-    shows "senderTransition ((SenderState St var_buffer var_c), (senderElemIn_As_I null null))
-         = (SenderState St var_buffer 3, (senderOut_Ds (Msg (Pair (last var_buffer) True))))"
-  oops
+    shows "senderTransition ((SenderState St var_buffer var_c), (senderElemIn_as_i null null))
+         = (SenderState St var_buffer 3, (senderOut_ds (Msg (Pair (last var_buffer) True))))"
+  apply(simp add: senderTransition_def)
+  sorry
 
 
 section \<open>Step-wise lemmata for the SPF\<close>
 
+(* Convert the SPF to step notation *)
+lemma senderSpf2Step: "senderSPF = spfConcOut (senderOut_ds null)\<cdot>(ReceiverStep (SenderState St []  0))"
+  sorry
+
 (* Line 33:  Sf -> St [buffer.size()>1 && i!=null] {as==false} / {buffer=buffer.butlast().prepend(i), c=3, ds=new Pair<>(buffer.butlast().last(),true)}; *)
-lemma step_0_0:
+lemma senderStep_0_0:
   assumes "(size var_buffer)>1 \<and> port_as=False"
-    shows "spfConcIn  (senderIn_As_I (Msg port_as) (Msg port_i))\<cdot>(SenderStep (SenderState Sf var_buffer var_c))
-         = spfConcOut (senderOut_Ds (Msg (Pair (last (butlast var_buffer)) True)))\<cdot>(SenderStep (SenderState St (prepend (butlast var_buffer) port_i) 3))"
-  oops
+    shows "spfConcIn  (senderIn_as_i (Msg port_as) (Msg port_i))\<cdot>(senderStep (SenderState Sf var_buffer var_c))
+         = spfConcOut (senderOut_ds (Msg (Pair (last (butlast var_buffer)) True)))\<cdot>(senderStep (SenderState St (prepend (butlast var_buffer) port_i) 3))"
+  apply(simp add: senderStep_def senderIn_as_i_def)
+  apply(rule da_h_stepI)
+  apply(auto simp add: daNextState_def daNextOutput_def assms)
+  (* TODO SWS: Manchmal fehlt noch das hier: *)
+  (*using assms by auto*)
+  sorry
 
 (* Line 35:  Sf -> St [buffer.size()=1 && i!=null] {as==false} / {buffer=buffer.butlast().prepend(i), c=3, ds=new Pair<>(i,true)}; *)
-lemma step_0_1:
+lemma senderStep_0_1:
   assumes "(size var_buffer)=1 \<and> port_as=False"
-    shows "spfConcIn  (senderIn_As_I (Msg port_as) (Msg port_i))\<cdot>(SenderStep (SenderState Sf var_buffer var_c))
-         = spfConcOut (senderOut_Ds (Msg (Pair port_i True)))\<cdot>(SenderStep (SenderState St (prepend (butlast var_buffer) port_i) 3))"
-  oops
+    shows "spfConcIn  (senderIn_as_i (Msg port_as) (Msg port_i))\<cdot>(senderStep (SenderState Sf var_buffer var_c))
+         = spfConcOut (senderOut_ds (Msg (Pair port_i True)))\<cdot>(senderStep (SenderState St (prepend (butlast var_buffer) port_i) 3))"
+  apply(simp add: senderStep_def senderIn_as_i_def)
+  apply(rule da_h_stepI)
+  apply(auto simp add: daNextState_def daNextOutput_def assms)
+  (* TODO SWS: Manchmal fehlt noch das hier: *)
+  (*using assms by auto*)
+  sorry
 
 (* Line 43:  Sf -> Sf [buffer.size()=0 && as!=null && i!=null] / {buffer=buffer.prepend(i), c=3, ds=new Pair<>(i,false)}; *)
-lemma step_0_2:
+lemma senderStep_0_2:
   assumes "(size var_buffer)=0"
-    shows "spfConcIn  (senderIn_As_I (Msg port_as) (Msg port_i))\<cdot>(SenderStep (SenderState Sf var_buffer var_c))
-         = spfConcOut (senderOut_Ds (Msg (Pair port_i False)))\<cdot>(SenderStep (SenderState Sf (prepend var_buffer port_i) 3))"
-  oops
+    shows "spfConcIn  (senderIn_as_i (Msg port_as) (Msg port_i))\<cdot>(senderStep (SenderState Sf var_buffer var_c))
+         = spfConcOut (senderOut_ds (Msg (Pair port_i False)))\<cdot>(senderStep (SenderState Sf (prepend var_buffer port_i) 3))"
+  apply(simp add: senderStep_def senderIn_as_i_def)
+  apply(rule da_h_stepI)
+  apply(auto simp add: daNextState_def daNextOutput_def assms)
+  (* TODO SWS: Manchmal fehlt noch das hier: *)
+  (*using assms by auto*)
+  sorry
 
 (* Line 45:  Sf -> Sf [buffer.size()>0 && c>0 && i!=null] {as==true} / {buffer=buffer.prepend(i), c=c-1}; *)
-lemma step_0_3:
+lemma senderStep_0_3:
   assumes "(size var_buffer)>0 \<and> var_c>0 \<and> port_as=True"
-    shows "spfConcIn  (senderIn_As_I (Msg port_as) (Msg port_i))\<cdot>(SenderStep (SenderState Sf var_buffer var_c))
-         = spfConcOut (senderOut_Ds null)\<cdot>(SenderStep (SenderState Sf (prepend var_buffer port_i) (var_c-1)))"
-  oops
+    shows "spfConcIn  (senderIn_as_i (Msg port_as) (Msg port_i))\<cdot>(senderStep (SenderState Sf var_buffer var_c))
+         = spfConcOut (senderOut_ds null)\<cdot>(senderStep (SenderState Sf (prepend var_buffer port_i) (var_c-1)))"
+  apply(simp add: senderStep_def senderIn_as_i_def)
+  apply(rule da_h_stepI)
+  apply(auto simp add: daNextState_def daNextOutput_def assms)
+  (* TODO SWS: Manchmal fehlt noch das hier: *)
+  (*using assms by auto*)
+  sorry
 
 (* Line 47:  Sf -> Sf [buffer.size()>0 && c=0 && i!=null] {as==true} / {buffer=buffer.prepend(i), c=3, ds=new Pair<>(buffer.last(),false)}; *)
-lemma step_0_4:
+lemma senderStep_0_4:
   assumes "(size var_buffer)>0 \<and> var_c=0 \<and> port_as=True"
-    shows "spfConcIn  (senderIn_As_I (Msg port_as) (Msg port_i))\<cdot>(SenderStep (SenderState Sf var_buffer var_c))
-         = spfConcOut (senderOut_Ds (Msg (Pair (last var_buffer) False)))\<cdot>(SenderStep (SenderState Sf (prepend var_buffer port_i) 3))"
-  oops
+    shows "spfConcIn  (senderIn_as_i (Msg port_as) (Msg port_i))\<cdot>(senderStep (SenderState Sf var_buffer var_c))
+         = spfConcOut (senderOut_ds (Msg (Pair (last var_buffer) False)))\<cdot>(senderStep (SenderState Sf (prepend var_buffer port_i) 3))"
+  apply(simp add: senderStep_def senderIn_as_i_def)
+  apply(rule da_h_stepI)
+  apply(auto simp add: daNextState_def daNextOutput_def assms)
+  (* TODO SWS: Manchmal fehlt noch das hier: *)
+  (*using assms by auto*)
+  sorry
 
 (* Line 34:  Sf -> St [buffer.size()>1] {as==false, i==null} / {buffer=buffer.butlast(), c=3, ds=new Pair<>(buffer.butlast().last(),true)}; *)
-lemma step_1_0:
+lemma senderStep_1_0:
   assumes "(size var_buffer)>1 \<and> port_as=False"
-    shows "spfConcIn  (senderIn_As_I (Msg port_as) null)\<cdot>(SenderStep (SenderState Sf var_buffer var_c))
-         = spfConcOut (senderOut_Ds (Msg (Pair (last (butlast var_buffer)) True)))\<cdot>(SenderStep (SenderState St (butlast var_buffer) 3))"
-  oops
+    shows "spfConcIn  (senderIn_as_i (Msg port_as) null)\<cdot>(senderStep (SenderState Sf var_buffer var_c))
+         = spfConcOut (senderOut_ds (Msg (Pair (last (butlast var_buffer)) True)))\<cdot>(senderStep (SenderState St (butlast var_buffer) 3))"
+  apply(simp add: senderStep_def senderIn_as_i_def)
+  apply(rule da_h_stepI)
+  apply(auto simp add: daNextState_def daNextOutput_def assms)
+  (* TODO SWS: Manchmal fehlt noch das hier: *)
+  (*using assms by auto*)
+  sorry
 
 (* Line 36:  Sf -> St [buffer.size()=1] {as==false, i==null} / {buffer=buffer.butlast()}; *)
-lemma step_1_1:
+lemma senderStep_1_1:
   assumes "(size var_buffer)=1 \<and> port_as=False"
-    shows "spfConcIn  (senderIn_As_I (Msg port_as) null)\<cdot>(SenderStep (SenderState Sf var_buffer var_c))
-         = spfConcOut (senderOut_Ds null)\<cdot>(SenderStep (SenderState St (butlast var_buffer) var_c))"
-  oops
+    shows "spfConcIn  (senderIn_as_i (Msg port_as) null)\<cdot>(senderStep (SenderState Sf var_buffer var_c))
+         = spfConcOut (senderOut_ds null)\<cdot>(senderStep (SenderState St (butlast var_buffer) var_c))"
+  apply(simp add: senderStep_def senderIn_as_i_def)
+  apply(rule da_h_stepI)
+  apply(auto simp add: daNextState_def daNextOutput_def assms)
+  (* TODO SWS: Manchmal fehlt noch das hier: *)
+  (*using assms by auto*)
+  sorry
 
 (* Line 38:  Sf -> Sf [buffer.size()=0 && as!=null] {i==null}; *)
-lemma step_1_2:
+lemma senderStep_1_2:
   assumes "(size var_buffer)=0"
-    shows "spfConcIn  (senderIn_As_I (Msg port_as) null)\<cdot>(SenderStep (SenderState Sf var_buffer var_c))
-         = spfConcOut (senderOut_Ds null)\<cdot>(SenderStep (SenderState Sf var_buffer var_c))"
-  oops
+    shows "spfConcIn  (senderIn_as_i (Msg port_as) null)\<cdot>(senderStep (SenderState Sf var_buffer var_c))
+         = spfConcOut (senderOut_ds null)\<cdot>(senderStep (SenderState Sf var_buffer var_c))"
+  apply(simp add: senderStep_def senderIn_as_i_def)
+  apply(rule da_h_stepI)
+  apply(auto simp add: daNextState_def daNextOutput_def assms)
+  (* TODO SWS: Manchmal fehlt noch das hier: *)
+  (*using assms by auto*)
+  sorry
 
 (* Line 40:  Sf -> Sf [buffer.size()>0 && c>0] {as==true, i==null} / {c=c-1}; *)
-lemma step_1_3:
+lemma senderStep_1_3:
   assumes "(size var_buffer)>0 \<and> var_c>0 \<and> port_as=True"
-    shows "spfConcIn  (senderIn_As_I (Msg port_as) null)\<cdot>(SenderStep (SenderState Sf var_buffer var_c))
-         = spfConcOut (senderOut_Ds null)\<cdot>(SenderStep (SenderState Sf var_buffer (var_c-1)))"
-  oops
+    shows "spfConcIn  (senderIn_as_i (Msg port_as) null)\<cdot>(senderStep (SenderState Sf var_buffer var_c))
+         = spfConcOut (senderOut_ds null)\<cdot>(senderStep (SenderState Sf var_buffer (var_c-1)))"
+  apply(simp add: senderStep_def senderIn_as_i_def)
+  apply(rule da_h_stepI)
+  apply(auto simp add: daNextState_def daNextOutput_def assms)
+  (* TODO SWS: Manchmal fehlt noch das hier: *)
+  (*using assms by auto*)
+  sorry
 
 (* Line 41:  Sf -> Sf [buffer.size()>0 && c=0] {as==true, i==null} / {c=3, ds=new Pair<>(buffer.last(),false)}; *)
-lemma step_1_4:
+lemma senderStep_1_4:
   assumes "(size var_buffer)>0 \<and> var_c=0 \<and> port_as=True"
-    shows "spfConcIn  (senderIn_As_I (Msg port_as) null)\<cdot>(SenderStep (SenderState Sf var_buffer var_c))
-         = spfConcOut (senderOut_Ds (Msg (Pair (last var_buffer) False)))\<cdot>(SenderStep (SenderState Sf var_buffer 3))"
-  oops
+    shows "spfConcIn  (senderIn_as_i (Msg port_as) null)\<cdot>(senderStep (SenderState Sf var_buffer var_c))
+         = spfConcOut (senderOut_ds (Msg (Pair (last var_buffer) False)))\<cdot>(senderStep (SenderState Sf var_buffer 3))"
+  apply(simp add: senderStep_def senderIn_as_i_def)
+  apply(rule da_h_stepI)
+  apply(auto simp add: daNextState_def daNextOutput_def assms)
+  (* TODO SWS: Manchmal fehlt noch das hier: *)
+  (*using assms by auto*)
+  sorry
 
 (* Line 44:  Sf -> Sf [buffer.size()=0 && i!=null] {as==null} / {buffer=buffer.prepend(i), c=3, ds=new Pair<>(i,false)}; *)
-lemma step_2_0:
+lemma senderStep_2_0:
   assumes "(size var_buffer)=0"
-    shows "spfConcIn  (senderIn_As_I null (Msg port_i))\<cdot>(SenderStep (SenderState Sf var_buffer var_c))
-         = spfConcOut (senderOut_Ds (Msg (Pair port_i False)))\<cdot>(SenderStep (SenderState Sf (prepend var_buffer port_i) 3))"
-  oops
+    shows "spfConcIn  (senderIn_as_i null (Msg port_i))\<cdot>(senderStep (SenderState Sf var_buffer var_c))
+         = spfConcOut (senderOut_ds (Msg (Pair port_i False)))\<cdot>(senderStep (SenderState Sf (prepend var_buffer port_i) 3))"
+  apply(simp add: senderStep_def senderIn_as_i_def)
+  apply(rule da_h_stepI)
+  apply(auto simp add: daNextState_def daNextOutput_def assms)
+  (* TODO SWS: Manchmal fehlt noch das hier: *)
+  (*using assms by auto*)
+  sorry
 
 (* Line 46:  Sf -> Sf [buffer.size()>0 && c>0 && i!=null] {as==null} / {buffer=buffer.prepend(i), c=c-1}; *)
-lemma step_2_1:
+lemma senderStep_2_1:
   assumes "(size var_buffer)>0 \<and> var_c>0"
-    shows "spfConcIn  (senderIn_As_I null (Msg port_i))\<cdot>(SenderStep (SenderState Sf var_buffer var_c))
-         = spfConcOut (senderOut_Ds null)\<cdot>(SenderStep (SenderState Sf (prepend var_buffer port_i) (var_c-1)))"
-  oops
+    shows "spfConcIn  (senderIn_as_i null (Msg port_i))\<cdot>(senderStep (SenderState Sf var_buffer var_c))
+         = spfConcOut (senderOut_ds null)\<cdot>(senderStep (SenderState Sf (prepend var_buffer port_i) (var_c-1)))"
+  apply(simp add: senderStep_def senderIn_as_i_def)
+  apply(rule da_h_stepI)
+  apply(auto simp add: daNextState_def daNextOutput_def assms)
+  (* TODO SWS: Manchmal fehlt noch das hier: *)
+  (*using assms by auto*)
+  sorry
 
 (* Line 48:  Sf -> Sf [buffer.size()>0 && c=0 && i!=null] {as==null} / {buffer=buffer.prepend(i), c=3, ds=new Pair<>(buffer.last(),false)}; *)
-lemma step_2_2:
+lemma senderStep_2_2:
   assumes "(size var_buffer)>0 \<and> var_c=0"
-    shows "spfConcIn  (senderIn_As_I null (Msg port_i))\<cdot>(SenderStep (SenderState Sf var_buffer var_c))
-         = spfConcOut (senderOut_Ds (Msg (Pair (last var_buffer) False)))\<cdot>(SenderStep (SenderState Sf (prepend var_buffer port_i) 3))"
-  oops
+    shows "spfConcIn  (senderIn_as_i null (Msg port_i))\<cdot>(senderStep (SenderState Sf var_buffer var_c))
+         = spfConcOut (senderOut_ds (Msg (Pair (last var_buffer) False)))\<cdot>(senderStep (SenderState Sf (prepend var_buffer port_i) 3))"
+  apply(simp add: senderStep_def senderIn_as_i_def)
+  apply(rule da_h_stepI)
+  apply(auto simp add: daNextState_def daNextOutput_def assms)
+  (* TODO SWS: Manchmal fehlt noch das hier: *)
+  (*using assms by auto*)
+  sorry
 
 (* Line 37:  Sf -> Sf [buffer.size()=0] {as==null, i==null}; *)
-lemma step_3_0:
+lemma senderStep_3_0:
   assumes "(size var_buffer)=0"
-    shows "spfConcIn  (senderIn_As_I null null)\<cdot>(SenderStep (SenderState Sf var_buffer var_c))
-         = spfConcOut (senderOut_Ds null)\<cdot>(SenderStep (SenderState Sf var_buffer var_c))"
-  oops
+    shows "spfConcIn  (senderIn_as_i null null)\<cdot>(senderStep (SenderState Sf var_buffer var_c))
+         = spfConcOut (senderOut_ds null)\<cdot>(senderStep (SenderState Sf var_buffer var_c))"
+  apply(simp add: senderStep_def senderIn_as_i_def)
+  apply(rule da_h_stepI)
+  apply(auto simp add: daNextState_def daNextOutput_def assms)
+  (* TODO SWS: Manchmal fehlt noch das hier: *)
+  (*using assms by auto*)
+  sorry
 
 (* Line 39:  Sf -> Sf [buffer.size()>0 && c>0] {as==null, i==null}; *)
-lemma step_3_1:
+lemma senderStep_3_1:
   assumes "(size var_buffer)>0 \<and> var_c>0"
-    shows "spfConcIn  (senderIn_As_I null null)\<cdot>(SenderStep (SenderState Sf var_buffer var_c))
-         = spfConcOut (senderOut_Ds null)\<cdot>(SenderStep (SenderState Sf var_buffer var_c))"
-  oops
+    shows "spfConcIn  (senderIn_as_i null null)\<cdot>(senderStep (SenderState Sf var_buffer var_c))
+         = spfConcOut (senderOut_ds null)\<cdot>(senderStep (SenderState Sf var_buffer var_c))"
+  apply(simp add: senderStep_def senderIn_as_i_def)
+  apply(rule da_h_stepI)
+  apply(auto simp add: daNextState_def daNextOutput_def assms)
+  (* TODO SWS: Manchmal fehlt noch das hier: *)
+  (*using assms by auto*)
+  sorry
 
 (* Line 42:  Sf -> Sf [buffer.size()>0 && c=0] {as==null, i==null} / {c=3, ds=new Pair<>(buffer.last(),false)}; *)
-lemma step_3_2:
+lemma senderStep_3_2:
   assumes "(size var_buffer)>0 \<and> var_c=0"
-    shows "spfConcIn  (senderIn_As_I null null)\<cdot>(SenderStep (SenderState Sf var_buffer var_c))
-         = spfConcOut (senderOut_Ds (Msg (Pair (last var_buffer) False)))\<cdot>(SenderStep (SenderState Sf var_buffer 3))"
-  oops
+    shows "spfConcIn  (senderIn_as_i null null)\<cdot>(senderStep (SenderState Sf var_buffer var_c))
+         = spfConcOut (senderOut_ds (Msg (Pair (last var_buffer) False)))\<cdot>(senderStep (SenderState Sf var_buffer 3))"
+  apply(simp add: senderStep_def senderIn_as_i_def)
+  apply(rule da_h_stepI)
+  apply(auto simp add: daNextState_def daNextOutput_def assms)
+  (* TODO SWS: Manchmal fehlt noch das hier: *)
+  (*using assms by auto*)
+  sorry
 
 (* Line 25:  St -> St [buffer.size()=0 && as!=null && i!=null] / {buffer=buffer.prepend(i), c=3, ds=new Pair<>(i,true)}; *)
-lemma step_4_0:
+lemma senderStep_4_0:
   assumes "(size var_buffer)=0"
-    shows "spfConcIn  (senderIn_As_I (Msg port_as) (Msg port_i))\<cdot>(SenderStep (SenderState St var_buffer var_c))
-         = spfConcOut (senderOut_Ds (Msg (Pair port_i True)))\<cdot>(SenderStep (SenderState St (prepend var_buffer port_i) 3))"
-  oops
+    shows "spfConcIn  (senderIn_as_i (Msg port_as) (Msg port_i))\<cdot>(senderStep (SenderState St var_buffer var_c))
+         = spfConcOut (senderOut_ds (Msg (Pair port_i True)))\<cdot>(senderStep (SenderState St (prepend var_buffer port_i) 3))"
+  apply(simp add: senderStep_def senderIn_as_i_def)
+  apply(rule da_h_stepI)
+  apply(auto simp add: daNextState_def daNextOutput_def assms)
+  (* TODO SWS: Manchmal fehlt noch das hier: *)
+  (*using assms by auto*)
+  sorry
 
 (* Line 27:  St -> Sf [buffer.size()>1 && i!=null] {as==true} / {buffer=buffer.butlast().prepend(i), c=3, ds=new Pair<>(buffer.butlast().last(),false)}; *)
-lemma step_4_1:
+lemma senderStep_4_1:
   assumes "(size var_buffer)>1 \<and> port_as=True"
-    shows "spfConcIn  (senderIn_As_I (Msg port_as) (Msg port_i))\<cdot>(SenderStep (SenderState St var_buffer var_c))
-         = spfConcOut (senderOut_Ds (Msg (Pair (last (butlast var_buffer)) False)))\<cdot>(SenderStep (SenderState Sf (prepend (butlast var_buffer) port_i) 3))"
-  oops
+    shows "spfConcIn  (senderIn_as_i (Msg port_as) (Msg port_i))\<cdot>(senderStep (SenderState St var_buffer var_c))
+         = spfConcOut (senderOut_ds (Msg (Pair (last (butlast var_buffer)) False)))\<cdot>(senderStep (SenderState Sf (prepend (butlast var_buffer) port_i) 3))"
+  apply(simp add: senderStep_def senderIn_as_i_def)
+  apply(rule da_h_stepI)
+  apply(auto simp add: daNextState_def daNextOutput_def assms)
+  (* TODO SWS: Manchmal fehlt noch das hier: *)
+  (*using assms by auto*)
+  sorry
 
 (* Line 28:  St -> St [buffer.size()>0 && c>0 && i!=null] {as==false} / {buffer=buffer.prepend(i), c=c-1}; *)
-lemma step_4_2:
+lemma senderStep_4_2:
   assumes "(size var_buffer)>0 \<and> var_c>0 \<and> port_as=False"
-    shows "spfConcIn  (senderIn_As_I (Msg port_as) (Msg port_i))\<cdot>(SenderStep (SenderState St var_buffer var_c))
-         = spfConcOut (senderOut_Ds null)\<cdot>(SenderStep (SenderState St (prepend var_buffer port_i) (var_c-1)))"
-  oops
+    shows "spfConcIn  (senderIn_as_i (Msg port_as) (Msg port_i))\<cdot>(senderStep (SenderState St var_buffer var_c))
+         = spfConcOut (senderOut_ds null)\<cdot>(senderStep (SenderState St (prepend var_buffer port_i) (var_c-1)))"
+  apply(simp add: senderStep_def senderIn_as_i_def)
+  apply(rule da_h_stepI)
+  apply(auto simp add: daNextState_def daNextOutput_def assms)
+  (* TODO SWS: Manchmal fehlt noch das hier: *)
+  (*using assms by auto*)
+  sorry
 
 (* Line 30:  St -> St [buffer.size()>0 && c=0 && i!=null] {as==false} / {buffer=buffer.prepend(i), c=3, ds=new Pair<>(buffer.last(),true)}; *)
-lemma step_4_3:
+lemma senderStep_4_3:
   assumes "(size var_buffer)>0 \<and> var_c=0 \<and> port_as=False"
-    shows "spfConcIn  (senderIn_As_I (Msg port_as) (Msg port_i))\<cdot>(SenderStep (SenderState St var_buffer var_c))
-         = spfConcOut (senderOut_Ds (Msg (Pair (last var_buffer) True)))\<cdot>(SenderStep (SenderState St (prepend var_buffer port_i) 3))"
-  oops
+    shows "spfConcIn  (senderIn_as_i (Msg port_as) (Msg port_i))\<cdot>(senderStep (SenderState St var_buffer var_c))
+         = spfConcOut (senderOut_ds (Msg (Pair (last var_buffer) True)))\<cdot>(senderStep (SenderState St (prepend var_buffer port_i) 3))"
+  apply(simp add: senderStep_def senderIn_as_i_def)
+  apply(rule da_h_stepI)
+  apply(auto simp add: daNextState_def daNextOutput_def assms)
+  (* TODO SWS: Manchmal fehlt noch das hier: *)
+  (*using assms by auto*)
+  sorry
 
 (* Line 32:  St -> Sf [buffer.size()=1 && i!=null] {as==true} / {buffer=buffer.butlast().prepend(i), c=3, ds=new Pair<>(i,false)}; *)
-lemma step_4_4:
+lemma senderStep_4_4:
   assumes "(size var_buffer)=1 \<and> port_as=True"
-    shows "spfConcIn  (senderIn_As_I (Msg port_as) (Msg port_i))\<cdot>(SenderStep (SenderState St var_buffer var_c))
-         = spfConcOut (senderOut_Ds (Msg (Pair port_i False)))\<cdot>(SenderStep (SenderState Sf (prepend (butlast var_buffer) port_i) 3))"
-  oops
+    shows "spfConcIn  (senderIn_as_i (Msg port_as) (Msg port_i))\<cdot>(senderStep (SenderState St var_buffer var_c))
+         = spfConcOut (senderOut_ds (Msg (Pair port_i False)))\<cdot>(senderStep (SenderState Sf (prepend (butlast var_buffer) port_i) 3))"
+  apply(simp add: senderStep_def senderIn_as_i_def)
+  apply(rule da_h_stepI)
+  apply(auto simp add: daNextState_def daNextOutput_def assms)
+  (* TODO SWS: Manchmal fehlt noch das hier: *)
+  (*using assms by auto*)
+  sorry
 
 (* Line 17:  St -> St [buffer.size()=0 && as!=null] {i==null}; *)
-lemma step_5_0:
+lemma senderStep_5_0:
   assumes "(size var_buffer)=0"
-    shows "spfConcIn  (senderIn_As_I (Msg port_as) null)\<cdot>(SenderStep (SenderState St var_buffer var_c))
-         = spfConcOut (senderOut_Ds null)\<cdot>(SenderStep (SenderState St var_buffer var_c))"
-  oops
+    shows "spfConcIn  (senderIn_as_i (Msg port_as) null)\<cdot>(senderStep (SenderState St var_buffer var_c))
+         = spfConcOut (senderOut_ds null)\<cdot>(senderStep (SenderState St var_buffer var_c))"
+  apply(simp add: senderStep_def senderIn_as_i_def)
+  apply(rule da_h_stepI)
+  apply(auto simp add: daNextState_def daNextOutput_def assms)
+  (* TODO SWS: Manchmal fehlt noch das hier: *)
+  (*using assms by auto*)
+  sorry
 
 (* Line 18:  St -> Sf [buffer.size()>1] {as==true, i==null} / {buffer=buffer.butlast(), c=3, ds=new Pair<>(buffer.butlast().last(),false)}; *)
-lemma step_5_1:
+lemma senderStep_5_1:
   assumes "(size var_buffer)>1 \<and> port_as=True"
-    shows "spfConcIn  (senderIn_As_I (Msg port_as) null)\<cdot>(SenderStep (SenderState St var_buffer var_c))
-         = spfConcOut (senderOut_Ds (Msg (Pair (last (butlast var_buffer)) False)))\<cdot>(SenderStep (SenderState Sf (butlast var_buffer) 3))"
-  oops
+    shows "spfConcIn  (senderIn_as_i (Msg port_as) null)\<cdot>(senderStep (SenderState St var_buffer var_c))
+         = spfConcOut (senderOut_ds (Msg (Pair (last (butlast var_buffer)) False)))\<cdot>(senderStep (SenderState Sf (butlast var_buffer) 3))"
+  apply(simp add: senderStep_def senderIn_as_i_def)
+  apply(rule da_h_stepI)
+  apply(auto simp add: daNextState_def daNextOutput_def assms)
+  (* TODO SWS: Manchmal fehlt noch das hier: *)
+  (*using assms by auto*)
+  sorry
 
 (* Line 20:  St -> St [buffer.size()>0 && c>0] {as==false, i==null} / {c=c-1}; *)
-lemma step_5_2:
+lemma senderStep_5_2:
   assumes "(size var_buffer)>0 \<and> var_c>0 \<and> port_as=False"
-    shows "spfConcIn  (senderIn_As_I (Msg port_as) null)\<cdot>(SenderStep (SenderState St var_buffer var_c))
-         = spfConcOut (senderOut_Ds null)\<cdot>(SenderStep (SenderState St var_buffer (var_c-1)))"
-  oops
+    shows "spfConcIn  (senderIn_as_i (Msg port_as) null)\<cdot>(senderStep (SenderState St var_buffer var_c))
+         = spfConcOut (senderOut_ds null)\<cdot>(senderStep (SenderState St var_buffer (var_c-1)))"
+  apply(simp add: senderStep_def senderIn_as_i_def)
+  apply(rule da_h_stepI)
+  apply(auto simp add: daNextState_def daNextOutput_def assms)
+  (* TODO SWS: Manchmal fehlt noch das hier: *)
+  (*using assms by auto*)
+  sorry
 
 (* Line 22:  St -> St [buffer.size()>0 && c=0] {as==false, i==null} / {c=3, ds=new Pair<>(buffer.last(),true)}; *)
-lemma step_5_3:
+lemma senderStep_5_3:
   assumes "(size var_buffer)>0 \<and> var_c=0 \<and> port_as=False"
-    shows "spfConcIn  (senderIn_As_I (Msg port_as) null)\<cdot>(SenderStep (SenderState St var_buffer var_c))
-         = spfConcOut (senderOut_Ds (Msg (Pair (last var_buffer) True)))\<cdot>(SenderStep (SenderState St var_buffer 3))"
-  oops
+    shows "spfConcIn  (senderIn_as_i (Msg port_as) null)\<cdot>(senderStep (SenderState St var_buffer var_c))
+         = spfConcOut (senderOut_ds (Msg (Pair (last var_buffer) True)))\<cdot>(senderStep (SenderState St var_buffer 3))"
+  apply(simp add: senderStep_def senderIn_as_i_def)
+  apply(rule da_h_stepI)
+  apply(auto simp add: daNextState_def daNextOutput_def assms)
+  (* TODO SWS: Manchmal fehlt noch das hier: *)
+  (*using assms by auto*)
+  sorry
 
 (* Line 24:  St -> Sf [buffer.size()=1] {as==true, i==null} / {buffer=buffer.butlast()}; *)
-lemma step_5_4:
+lemma senderStep_5_4:
   assumes "(size var_buffer)=1 \<and> port_as=True"
-    shows "spfConcIn  (senderIn_As_I (Msg port_as) null)\<cdot>(SenderStep (SenderState St var_buffer var_c))
-         = spfConcOut (senderOut_Ds null)\<cdot>(SenderStep (SenderState Sf (butlast var_buffer) var_c))"
-  oops
+    shows "spfConcIn  (senderIn_as_i (Msg port_as) null)\<cdot>(senderStep (SenderState St var_buffer var_c))
+         = spfConcOut (senderOut_ds null)\<cdot>(senderStep (SenderState Sf (butlast var_buffer) var_c))"
+  apply(simp add: senderStep_def senderIn_as_i_def)
+  apply(rule da_h_stepI)
+  apply(auto simp add: daNextState_def daNextOutput_def assms)
+  (* TODO SWS: Manchmal fehlt noch das hier: *)
+  (*using assms by auto*)
+  sorry
 
 (* Line 26:  St -> St [buffer.size()=0 && i!=null] {as==null} / {buffer=buffer.prepend(i), c=3, ds=new Pair<>(i,true)}; *)
-lemma step_6_0:
+lemma senderStep_6_0:
   assumes "(size var_buffer)=0"
-    shows "spfConcIn  (senderIn_As_I null (Msg port_i))\<cdot>(SenderStep (SenderState St var_buffer var_c))
-         = spfConcOut (senderOut_Ds (Msg (Pair port_i True)))\<cdot>(SenderStep (SenderState St (prepend var_buffer port_i) 3))"
-  oops
+    shows "spfConcIn  (senderIn_as_i null (Msg port_i))\<cdot>(senderStep (SenderState St var_buffer var_c))
+         = spfConcOut (senderOut_ds (Msg (Pair port_i True)))\<cdot>(senderStep (SenderState St (prepend var_buffer port_i) 3))"
+  apply(simp add: senderStep_def senderIn_as_i_def)
+  apply(rule da_h_stepI)
+  apply(auto simp add: daNextState_def daNextOutput_def assms)
+  (* TODO SWS: Manchmal fehlt noch das hier: *)
+  (*using assms by auto*)
+  sorry
 
 (* Line 29:  St -> St [buffer.size()>0 && c>0 && i!=null] {as==null} / {buffer=buffer.prepend(i), c=c-1}; *)
-lemma step_6_1:
+lemma senderStep_6_1:
   assumes "(size var_buffer)>0 \<and> var_c>0"
-    shows "spfConcIn  (senderIn_As_I null (Msg port_i))\<cdot>(SenderStep (SenderState St var_buffer var_c))
-         = spfConcOut (senderOut_Ds null)\<cdot>(SenderStep (SenderState St (prepend var_buffer port_i) (var_c-1)))"
-  oops
+    shows "spfConcIn  (senderIn_as_i null (Msg port_i))\<cdot>(senderStep (SenderState St var_buffer var_c))
+         = spfConcOut (senderOut_ds null)\<cdot>(senderStep (SenderState St (prepend var_buffer port_i) (var_c-1)))"
+  apply(simp add: senderStep_def senderIn_as_i_def)
+  apply(rule da_h_stepI)
+  apply(auto simp add: daNextState_def daNextOutput_def assms)
+  (* TODO SWS: Manchmal fehlt noch das hier: *)
+  (*using assms by auto*)
+  sorry
 
 (* Line 31:  St -> St [buffer.size()>0 && c=0 && i!=null] {as==null} / {buffer=buffer.prepend(i), c=3, ds=new Pair<>(buffer.last(),true)}; *)
-lemma step_6_2:
+lemma senderStep_6_2:
   assumes "(size var_buffer)>0 \<and> var_c=0"
-    shows "spfConcIn  (senderIn_As_I null (Msg port_i))\<cdot>(SenderStep (SenderState St var_buffer var_c))
-         = spfConcOut (senderOut_Ds (Msg (Pair (last var_buffer) True)))\<cdot>(SenderStep (SenderState St (prepend var_buffer port_i) 3))"
-  oops
+    shows "spfConcIn  (senderIn_as_i null (Msg port_i))\<cdot>(senderStep (SenderState St var_buffer var_c))
+         = spfConcOut (senderOut_ds (Msg (Pair (last var_buffer) True)))\<cdot>(senderStep (SenderState St (prepend var_buffer port_i) 3))"
+  apply(simp add: senderStep_def senderIn_as_i_def)
+  apply(rule da_h_stepI)
+  apply(auto simp add: daNextState_def daNextOutput_def assms)
+  (* TODO SWS: Manchmal fehlt noch das hier: *)
+  (*using assms by auto*)
+  sorry
 
 (* Line 19:  St -> St [buffer.size()=0] {as==null, i==null}; *)
-lemma step_7_0:
+lemma senderStep_7_0:
   assumes "(size var_buffer)=0"
-    shows "spfConcIn  (senderIn_As_I null null)\<cdot>(SenderStep (SenderState St var_buffer var_c))
-         = spfConcOut (senderOut_Ds null)\<cdot>(SenderStep (SenderState St var_buffer var_c))"
-  oops
+    shows "spfConcIn  (senderIn_as_i null null)\<cdot>(senderStep (SenderState St var_buffer var_c))
+         = spfConcOut (senderOut_ds null)\<cdot>(senderStep (SenderState St var_buffer var_c))"
+  apply(simp add: senderStep_def senderIn_as_i_def)
+  apply(rule da_h_stepI)
+  apply(auto simp add: daNextState_def daNextOutput_def assms)
+  (* TODO SWS: Manchmal fehlt noch das hier: *)
+  (*using assms by auto*)
+  sorry
 
 (* Line 21:  St -> St [buffer.size()>0 && c>0] {as==null, i==null} / {c=c-1}; *)
-lemma step_7_1:
+lemma senderStep_7_1:
   assumes "(size var_buffer)>0 \<and> var_c>0"
-    shows "spfConcIn  (senderIn_As_I null null)\<cdot>(SenderStep (SenderState St var_buffer var_c))
-         = spfConcOut (senderOut_Ds null)\<cdot>(SenderStep (SenderState St var_buffer (var_c-1)))"
-  oops
+    shows "spfConcIn  (senderIn_as_i null null)\<cdot>(senderStep (SenderState St var_buffer var_c))
+         = spfConcOut (senderOut_ds null)\<cdot>(senderStep (SenderState St var_buffer (var_c-1)))"
+  apply(simp add: senderStep_def senderIn_as_i_def)
+  apply(rule da_h_stepI)
+  apply(auto simp add: daNextState_def daNextOutput_def assms)
+  (* TODO SWS: Manchmal fehlt noch das hier: *)
+  (*using assms by auto*)
+  sorry
 
 (* Line 23:  St -> St [buffer.size()>0 && c=0] {as==null, i==null} / {c=3, ds=new Pair<>(buffer.last(),true)}; *)
-lemma step_7_2:
+lemma senderStep_7_2:
   assumes "(size var_buffer)>0 \<and> var_c=0"
-    shows "spfConcIn  (senderIn_As_I null null)\<cdot>(SenderStep (SenderState St var_buffer var_c))
-         = spfConcOut (senderOut_Ds (Msg (Pair (last var_buffer) True)))\<cdot>(SenderStep (SenderState St var_buffer 3))"
-  oops
+    shows "spfConcIn  (senderIn_as_i null null)\<cdot>(senderStep (SenderState St var_buffer var_c))
+         = spfConcOut (senderOut_ds (Msg (Pair (last var_buffer) True)))\<cdot>(senderStep (SenderState St var_buffer 3))"
+  apply(simp add: senderStep_def senderIn_as_i_def)
+  apply(rule da_h_stepI)
+  apply(auto simp add: daNextState_def daNextOutput_def assms)
+  (* TODO SWS: Manchmal fehlt noch das hier: *)
+  (*using assms by auto*)
+  sorry
 
 
 end
